# Original Question

There is a spin 1/2 particle with magnetic moment mu (= gamma*Sz), aligned with a magnetic field pointing in the +Z direction. Suddenly, the magnetic field is turned off, and another one is turned on along the +Y direction; both fields have the same magnitude, B. The average of the z-component of the particle’s moment starts oscillating. What is its oscillation frequency?

---

# DeepSeek response (via openrouter)



---

# DeepSeek reasoning (via openrouter)

To solve for the oscillation frequency of the average z-component of the particle's magnetic moment when the magnetic field is switched from the z-direction to the y-direction (while keeping the same magnitude $B$), we need to solve for the time evolution of the quantum state of a spin-1/2 particle.

Initially, the magnetic field points along the $+Z$ direction and has a magnitude of $B$, so the Hamiltonian can be written as:
$$
H_1 = -\vec{\mu} \cdot \vec{B} = -\mu B \hat{z} \cdot \hat{z} = -\mu B,
$$
where $\vec{\mu} = \gamma \vec{S}$ is defined such that $\vec{\mu} = \gamma \vec{S}$ with $\gamma$ being the gyromagnetic ratio and $\vec{S}$ being the spin angular momentum operator (where $\vec{S} = (\hbar/2) \vec{\sigma}$ for a spin-1/2 particle where $\vec{\sigma}$ is the Pauli spin matrices vector).

However, the problem statement mentions that the magnetic moment is given by $\mu = \gamma S_z$, which appears to be a bit imprecise (since $\mu$ should be a vector quantity). A more standard way to express the magnetic moment for a spin-1/2 particle is:
$$
\vec{\mu} = \gamma \vec{S} = \gamma \frac{\hbar}{2} \vec{\sigma}.
$$
where $\vec{\sigma} = (\sigma_x, \sigma_y, \sigma_z)$ are the Pauli matrices. For a spin $1/2$ particle, the $z$-component of the magnetic moment is:
$$
\mu_z = \gamma S_z,
$$
where $S_z$ is the $z$-component of the spin angular momentum given by:
$$
S_z = \frac{\hbar}{2}\sigma_z.
$$
So, the total Hamiltonian while the magnetic field is in the $z$-direction can be rewritten as:
$$
H_1 = -\vec{\mu} \cdot \vec{B} = -(\gamma S_z) B,
$$
since:
$$
\vec{\mu} \cdot \vec{B} = \gamma (S_x \hat{x} + S_y \hat{y} + S_z \hat{z}) \cdot B \hat{z} = \gamma B S_z.
$$
So, $H_1 = - (\gamma B S_z)$, which implies:
$$
H_implies = - \gamma B S_z = - \gamma B \left(\frac{\hbar}{2} \sigma_z \right) = -\frac{\gamma B \hbar}{2} \sigma_z,
$$
where $\sigma_z = \begin{pmatrix} 1 & 0 \\ 0 & -1 \end{pmatrix}$ represents the $\sigma_z$ Pauli matrix.

However, the question states that the field is "aligned with a magnetic field pointing in the $+Z$ direction." This means that the initial Hamiltonian could possibly be simplified as:
$$
H_1 = - \mu B,
$$
if $\mu$ here means $\mu_z = \gamma s_z$, where $s_z$ is the eigenvalue of $S_z$. However, that part might be a bit confusing because the Hamiltonian should normally be written as $H_1 = - \gamma B S_z$.

Given that the question states that the particle is "aligned" with the magnetic field in the $+Z$ direction, it seems that the initial state should be an eigenstate of $S_z$ such that the particle has a "positive" spin component along the $Z$ direction (i.e., the spin points in the same direction as the magnetic field). The Hamiltonian previously described is diagonalized by the $|+\rangle$ (spin-up state along $z$, usually represented as $|\uparrow\rangle$) and $|-\rangle$ (spin-down state along $z$, usually represented as $|\downarrow\rangle$) states where $|\uparrow\rangle = |1/2,1/2\rangle = \begin{pmatrix} 1 \\ 0 \end{pmatrix}$ and $|\downarrow\rangle = \begin{pmatrix} 0 \\ 1 \end{pmatrix}$.

Since the particle is "aligned" with $B\hat{z}$, let us assume that the initial quantum state of the particle is in the spin-up state along $z$:
$$
|\psi(0)\rangle = |\uparrow\rangle = \begin{pmatrix} 1 \\ 0 \end{pmatrix}.
$$
However, another part of the question states that "suddenly" the magnetic field is turned off and another one is turned on along the $+Y$ direction with the same magnitude $B$. Therefore, the new Hamiltonian after this change becomes:
$$
H_2 = - \vec{\mu} \cdot \vec{B} = - \gamma \vec{S} \cdot B\hat{y} = - \gamma B S_y,
$$
where $S_y = \frac{\hbar}{2}\sigma_y$ and:
$$\sigma_y = \begin{pmatrix} 0 & -i \\ i & 0 \end{pmatrix}.$$
So, the Hamiltonian thus becomes:
$$
H_2 = - \gamma B \left(\frac{\hbar}{2}\begin{pmatrix} 0 & -i \\ i & 0\end{pmatrix}\right) = -\frac{\gamma B\hbar}{2} \begin{pmatrix} 0 & -i \\ i & 0\end{pmatrix}.
$$
Let denote $\omega = \frac{\gamma B\hbar}{2}$, so that:
$$\omega = \frac{\gamma B \hbar}{2},
$$
which makes:
$$
H_2 = -\omega \begin{pmatrix} 0 & -i \\ i & 0 \end{pmatrix} = \begin{pmatrix} 0 & i\omega \\ -i\omega & 0 \end{pmatrix}.
$$

However, what we need is to solve for the time evolution of the initial state $|\psi(0)\rangle$ under the new Hamiltonian $H_2$. Using Schrödinger's equation $i\hbar \frac{\partial |\psi(t)\rangle}{\partial t} = H_2|\psi(t)\rangle$, the state $|\psi(t)\rangle$ evolves as:
$$
|\psi(t)\rangle = e^{-i H_2 t / \hbar} |\psi(0)\rangle.
$$

To solve for $e^{-i H_2 t / \hbar}$, first make $H_2$ explicit again explicitly:
$$
H_2 = \begin{pmatrix} 0 & i\omega \\ -i\omega & 0 \end{pmatrix}.
$$
To make the exponential $e^{-i H_2 t / \hbar}$ more tractable, it is helpful to find the eigenvalues and eigenvectors for $H_2$. However, a shortcut might be to solve for the Hamiltonian explicitly by diagonalizing it:
$$
\begin{pmatrix} 0 & i\omega \\ -i\omega & 0 \end{pmatrix}.
$$
To find the eigenvalues $\lambda$ of $H_2$, solve for:
$$
\det(H_2 - \lambda I) = \det \begin{pmatrix} -\lambda & i\omega \\ -i\omega & -\lambda \end{pmatrix} = \lambda^2 - (i\omega)(-i\omega) = \lambda^2 - \omega^2.
$$
Thus, $\lambda = \pm \omega$, where $\omega = \frac{\gamma B \hbar}{2}$.

For $\lambda_1 = \omega$, solve for the eigenvector $|+\omega\rangle$ such that:
$$
\begin{pmatrix} 0 & i\omega \\ -i\omega & 0 \end{pmatrix} \begin{pmatrix} a \\ b \end{pmatrix} = \omega \begin{pmatrix} a \\ b \end{pmatrix}.
$$
This gives us the system of equations:
$$
i\omega b = \omega a \implies b = -ia,
\\
-i\omega a = \omega b \implies a = ib,
$$
which implies $b = -i a$. Such an eigenpair thus can be normalized as:
$$
|+\omega\rangle = \frac{1}{\sqrt{2}} \begin{pmatrix} 1 \\ -iy \end{pmatrix}.
$$
Normalization gives us:
$$
\left|\begin{pmatrix} 1 \\ -i \end{pmatrix}\right|^2 = 1^2 + |-i|^2 = 1 + 1 = 2.
$$
Therefore, the normalized eigenvector for the eigenvalue $\omega$ is:
$$
|+\omega\rangle = \frac{1}{\sqrt{2}} \begin{pmatrix}1 \\ -i\end{pmatrix}.
$$
For $\lambda_2 = -\omega$, solve for the eigenvector $|-\omega\rangle$ such that:
$$
\begin{pmatrix} 0 & i\omega \\ -i \omega & 0 \end{pmatrix} \begin{pmatrix}c\\d\end{pmatrix} = -\omega \begin{pmatrix}c\\d\end{pmatrix}.
$$
This gives us the system of equations:
$$
i\omega d = -\omega c \implies d = ic,
\\
-i\omega c = -\omega d \implies c = -id,
$$
which implies $d = i c$. Such an eigenpair can thus be:
$$
|-\omega\rangle = \frac{1}{\sqrt{2}} \begin{pmatrix} 1 \\ i \end{pmatrix}.
$$
Similarly, normalization yields:
$$
\left|\begin{pmatrix} 1 \\ i \end{pmatrix}\right|^2 = 1^2 + |i|^2 = 1 + (+1) = 2,
$$
so the normalized eigenvector for the eigenvalue $-\omega$ is:
$$
|-\omega\rangle = \frac{1}{\sqrt{2}} \begin{pmatrix} 1 \\ i \end{pmatrix}.
$$

#### Expressing Initial State in Eigenbasis of $H_2$

The initial state $|\psi(0)\rangle$ can be written in the eigenbasis of $|-y\rangle$ and $|+y\rangle$, which are the spin eigenstates along the $y$ basis where $|+y\rangle$ has spin "up" along $y$ and $|-y\rangle$ has spin "down" along $y$. However, in this case, the eigenstates we need are the eigenvectors of $H_2$. 

However, there seems to be a slight confusion here, because the eigenvectors we calculated previously are actually the eigenvectors for $\sigma_y$. However, the eigenvectors for $H_2$ are the same as those of $S_y$ (since $H_2 = -\gamma B S_y$, which is directly proportional to $S_y$).

Recall that the eigenstates of $S_y$ for eigenvalues $\pm \hbar/2$ are:
$$
|+\rangle_y = \frac{1}{\sqrt{2}} \begin{pmatrix} 1 \\ i \end{pmatrix} \text{ (eigenvalue $+\hbar / 2$)}
$$
and
$$
|-\rangle_y = \frac{1}{\sqrt{2}} \begin{pmatrix} 1 \\ -i \end{pmatrix} \text{ (eigenvalue $-\hbar / 2$)}.
$$
However, this was calculated from $S_y = \frac{\hbar}{2} \sigma_y$, thus:
$$
\sigma_y | \pm \rangle_y = \pm |\pm\rangle_y,
$$
which implies:
$$
S_y | \pm \rangle_y = \pm \frac{\hbar}{2} | \pm \rangle_y .
$$
Hence, the eigenvectors for $H_2$ which should be the eigenvectors for $S_y$. However, the notation might be a bit confusing here because $H_2 = - \gamma B S_y$. Thus, the eigenvalues of $H_2$ should be:
$$
H_2|\pm\rangle_y = - \gamma B S_y |\pm\rangle_y,
$$
which yields:
$$
H_2 |+\rangle_y = - \gamma B S_y |+\rangle_y = -\gamma B \left(\frac{\hbar}{2}\right)|+\rangle_y = -\frac{\gamma B \hbar}{2} |+\rangle_y,
$$
similarly:
$$
H_2|-\rangle_y = - \gamma B S_y |-\rangle_y = -\gamma B \left(-\frac{\hbar}{2} \right)|-\rangle_y = \frac{\gamma B \hbar}{2} |-\rangle_y,
$$
which shows that the eigenstates $|\pm\rangle_y$ of $H_2$ correspond to eigenvalues:
$$
\mp \frac{\gamma B\hbar}{2} = \mp \omega.
$$
Hence, $|+\rangle_y$ has an eigenvalue $-\omega$ for $H_2$, whereas $|-\rangle_y$ has an eigenvalue $+\omega$ for $H_2$. 

Let us express $|\psi(0)\rangle$ in terms of the $|+\rangle_y$ and $|-\rangle_y$ basis states (since this is the natural basis here):
$$
|\psi(0)\rangle = |\uparrow\rangle = \begin{pmatrix}1\\0\end{pmatrix} = \alpha |+\rangle_y + \beta |-\rangle_y,
$$
where:
$$
|+\rangle_y = \frac{1}{\sqrt{2}} \begin{pmatrix} 1 \\ i \end{pmatrix} = \frac{1}{\sqrt{2}}(|\uparrow\rangle + i |\downarrow\rangle ) ,
$$
$$
|-\rangle_y = \frac{1}{\sqrt{2}} \begin{pmatrix} 1 \\ -i \end{pmatrix} = \frac{1}{\sqrt{2}}(|\uparrow\rangle - i |\downarrow\rangle).
$$
To find $\alpha$ and $\beta$, solve:
$$
\begin{pmatrix} 1 \\ 0 \end{pmatrix} = \alpha \frac{1}{\sqrt{2}}\begin{pmatrix}1\\i\end{pmatrix} + \beta \frac{1}{\sqrt{2}}\begin{pmatrix}1\\-i\end{pmatrix} = \frac{1}{\sqrt{2}} \begin{pmatrix} \alpha + \beta \\ i\alpha - i \beta \end{pmatrix}.
$$
This implies solving the simultaneous equations:
$$
\frac{1}{\sqrt{2}} (\alpha + \beta) = 1,
$$
$$
\frac{1}{\sqrt{2}} (i \alpha - i \beta) = 0.
$$
The second equation leads to $\alpha = \beta$, so substituting this into the first equation yields:
$$
\frac{1}{\sqrt{2}} (\alpha + \alpha) = 1 \implies \frac{2\alpha}{\sqrt{2}} = 1 \implies \alpha = \frac{\sqrt{2}}{2} = \frac{1}{\sqrt{2}}.
$$
And hence:
$$
\beta = \frac{1}{\sqrt{2}}.
$$

Therefore:
$$
|\psi(0)\rangle = \frac{1}{\sqrt{2}} |+\rangle_y + \frac{1}{\sqrt{2}}|-\rangle_y.
$$
Now, given that $|+\rangle_y$ and $|-\rangle_y$ are eigenstates of $H_2$ with eigenvalues $-\omega$ and $\omega$ respectively, the time evolution can be computed individually for each part of the state:
$$
|\psi(t)\rangle = \frac{1}{\sqrt{2}} e^{-i H_2 t / \hbar} |+\rangle_y + \frac{1}{\sqrt{2}} e^{-i H_2 t / \hbar} |-\rangle_y,
$$
where $e^{-iH_2 t / \hbar}$ acts on the eigenstates $|+\rangle_y$ and $|-\rangle_y$ such that:
$$
H_2 |+\rangle_y = -\omega |+\rangle_y \Longrightarrow e^{-i H_2 t / \hbar} |+\rangle_y = e^{-i (-\omega) t / \hbar} |+\rangle_y = e^{i \omega t / \hbar} |+\rangle_y.
$$
$$
H_2 |-\rang_y = \omega |-\rangle_y \Longrightarrow e^{-i H_2 t / \hbar} |-\rangle_y = e^{-i \omega t / \hbar} |-\rangle_y.
$$
Note that $ \omega = \frac{\gamma B\hbar}{2}$, so $\frac{\omega}{\hbar} = \frac{\gamma B}{2}$.

Thus, the state evolves as:
$$
|\psi(t)\rangle = \frac{1}{\sqrt{2}} e^{i \omega t / \hbar} |+\rangle_y + \frac{1}{\sqrt{2}} e^{-i \omega t / \hbar} |-\rangle_y .
$$
$$
= \frac{1}{\sqrt{2}} e^{i \omega t / \hbar} \cdot \frac{1}{\sqrt{2}}(|\uparrow\rangle + i |\downarrow\rangle) + \frac{1}{\sqrt{2}} e^{-i \omega t / \hbar} \cdot \frac{1}{\sqrt{2}}(|\uparrow\rangle - i |\downarrow\rangle).
$$
$$
= \frac{1}{\sqrt{2}} e^{i \omega t / \hbar} \left(\frac{1}{\sqrt{2}}|\uparrow\rangle + \frac{i}{\sqrt{2}}|\downarrow\rangle\right) + \frac{1}{\sqrt{2}} e^{-i \omega t / \hbar} \left(\frac{1}{\sqrt{2}}|\uparrow\rangle - \frac{i}{\sqrt{2}}|\downarrow\rangle\rangle\right).
$$
$$
= \frac{e^{i \omega t / \hbar} + e^{-i \omega t / \hbar}}{2} |\uparrow\rangle + \frac{i(e^{i \omega t / \hbar} - e^{-i \omega t / \hbar})}{2} |\downarrow\rangle.
$$
Using the identity $\cos x = \frac{e^{ix} + e^{-ix}}{2}$ and $\sin x = \frac{e^{ix} - e^{-ix}}{2i}$:
$$
|\psi(t)\rangle = \cos\bigg(\frac{\omega}{\hbar}t\bigg)|\uparrow\rangle - \sin\bigg(\frac{\omega}{\hbar}t\bigg)|\downarrow\rangle.
$$
However, the question asks us to find the average value for the magnetic moment in the $z$ direction, specifically:
$$
\langle \mu_z \rangle = \gamma \langle S_z \rangle.
$$
Thus, we need to compute:
$$
\langle S_z \rangle = \langle \psi(t) | S_z | \psi(t) \rangle,
$$
where:
$$
S_z = \frac{\hbar}{2} \sigma_z = \frac{\hbar}{2} \begin{pmatrix} 1 & 0 \\ 0 & -1\end{pmatrix}.
$$
The state $|\psi(t)\rangle$, written explicitly as a column vector, is:
$$\begin{align*}
|\psi(t)\rangle &= \cos\left(\frac{\omega}{\hbar}t\right) \begin{pmatrix} 1 \\ 0 \end{pmatrix} - \sin\Big(\frac{\omega}{\hbar}t\Big) \begin{pmatrix} 0 \\ 1 \end{pmatrix} = \cos\left(\frac{\omega}{\hbar}t\right) \begin{pmatrix} 1 \\ 0 \end{pmatrix} + \sin\Big(\frac{\omega}{\hbar}t\Big) \begin{pmatrix} 0 \\ -1 \end{pmatrix} \\
&= \begin{pmatrix} \cos\left(\frac{\omega}{\hbar}t\right) \\ -\sin

---

