# Original Question

Calculate the eigenvector of a quantum mechanical operator $\vec{P}$ for a muon along an arbitrary direction $\vec{n}$ lying in the x-z plane corresponding to the eigenvalue $+\hbar/2$. Given the $X-$component, $P_x$ of the operator $P$ as $\hbar/2$ times a 2 by 2 square matrix having elements in the first row as $(0 1)$, and that in the second row as $(1, 0)$. The $Y-$component, $P_y$ of the operator is given by the product of $\hbar/2$ and a 2 by 2 square matrix having elements in the first row as $(0, -i)$, and that in the second row as $(i, 0)$. Finally, the $Z-$component, $P_z$ of the operator is given by the product of $\hbar/2$  and another 2 by 2 square matrix having elements in the first row as $(1, 0)$, and that in the second row as $(0, -1)$.  What are the elements of the normalized eigenvector? 


---

# DeepSeek response (via openrouter)



---

# DeepSeek reasoning (via openrouter)

To solve for the eigenvector of the quantum mechanical operator $\vec{P}$ for a muon (which seems to describe a spin-$\frac{1}{2}$ particle) along an arbitrary direction $\vec{n}$ in the $x$-$z$ plane corresponding to the eigenvalue $+\frac{\hbar}{2}$, we need to first identify the given operator components $P_x$, $P_y$, and $P_z$.

The question gives us:

$$
P_x = \frac{\hbar}{2} \begin{pmatrix}
0 & 1 \\
1 & 0
\end{pmatrix}.
$$
$$
P_y = \frac{\hbar}{2} \begin{pmatrix}
0 & -i \\
i & 0
\end{pmatrix}.
$$
$$
P_z = \frac{\hbar}{2} \begin{pmatrix}
1 & 0 \\
0 & -1
\end{pmatrix}.
$$

The question mentions that $\vec{n}$ is a unit vector lying in the $x$-$z$ plane. An arbitrary vector in the $x$-$z$ plane can be expressed as $\vec{n} = \sin\theta \hat{i} + 0 \hat{j} + \cos\theta \hat{k}$ where $\theta$ is the angle that the vector $\vec{n}$ makes with the $z$-axis such that:
$$
\vec{n} = \sin\theta \hat{x} + \cos\theta \hat{z}.
$$

The operator $\vec{P} \cdot \vec{n}$ thus represents the component of the operator $\vec{P}$ along the direction $\vec{n}$:
$$
\vec{P} \cdot \vec{n} = P_x \sin\theta + P_y \cdot 0 + P_z \cos\theta = P_x \sin\theta + P_z \cos\theta.
$$

Let us substitute the given $P_x$ and $P_z$ expressions:
$$
\vec{P} \cdot \vec{n} = \sin\theta \cdot \frac{\hbar}{2} \begin{pmatrix}
0 & 1 \\
1 & 0
\end{pmatrix} + \cos\theta \cdot \frac{\hbar}{2} \begin{pmatrix}
1 & 0 \\
0 & -1
\end{pmatrix}.
$$
Thus,
$$
\vec{P} \cdot \vec{n} = \frac{\hbar}{2} \sin\theta \begin{pmatrix}
0 & 1\\
1 & 0
\end{pmatrix} + \frac{\hbar}{2} \cos\theta \begin{pmatrix}
1 & 0 \\
0 & -1
\end{pmatrix}.
$$
$$
= \frac{\hbar}{2}\left(\sin\theta \cdot \begin{pmatrix}
0 & 1\\
1 & 0\end{pmatrix} + \cos\theta \cdot \begin{pmatrix}
1 & 0 \\
0 & -1
\end{pmatrix}\right).
$$
$$
= \frac{\hbar}{2} \left(\begin{pmatrix}
0 & \sin\theta\\
\sin\theta & 0
\end{pmatrix} + \begin{pmatrix}
\cos\theta & 0\\
0 & -\cos\theta
\end{pmatrix}\right).
$$
$$
= \frac{\hbar}{2} \begin{pmatrix}
0 + \cos\theta & \sin\theta + 0 \\
\sin\theta + 0 & 0 - \cos\theta
\end{pmatrix}.
$$
$$
\sqrt[\phantom{}]{\phantom{}}
= \frac{\hbar}{2} \begin{pmatrix}
\cos\theta & \sin\theta\\
\sin\theta & -\cos\theta
\end{pmatrix}.
$$

We need to find the eigenvector for this matrix corresponding to the eigenvalue $+\frac{\hbar}{2}$. Let us solve for the eigenvalues of the following matrix first:
$$
\frac{\hbar}{2} \begin{pmatrix}
\cos\theta & \sin\theta \\
sin\theta & -\cos\theta
\end{pmatrix}.
$$
Let us denote the matrix without the constant factor $\frac{\hbar}{2}$:
$$
A = \begin{pmatrix}
\cos\theta & \sin\theta\\
\sin\theta & - \cos\theta
\end{pmatrix}.
$$

The full operator thus becomes $\vec{P} \cdot \vec{n} = \frac{\hbar}{2} A$. To solve for eigenvectors and eigenvalues of $\vec{P} \cdot \vec{n}$, let us find the eigenvalues $\lambda$ such that:
$$
\vec{P} \cdot \vec{n} \psi = \lambda \psi.
$$
where $\psi=\begin{pmatrix} a \\ b \end{pmatrix}$ is an eigenvector such that:
$$
\frac{\hbar}{2} \begin{pmatrix}
\cos\theta & \sin\theta\\
\sin\theta & -\cos\theta
\end{pmatrix} \begin{pmatrix} a \\ b \end{pmatrix} = \lambda \begin{pmatrix} a \\ b \end{pmatrix}.
$$
However, the question states that the desired eigenvalue we need is $+\frac{\hbar}{2}$ for the eigenvector:
$$
\frac{\hbar}{2} \begin{pmatrix}
cos\theta & \sin\theta\\
\sin\theta & -cos\theta
\end{pmatrix} \begin{pmatrix} a \\ b \end{pmatrix} = \frac{\hbar}{2} \begin{pmatrix} a \\ b \end{pmatrix}.
$$
This implies that our task is to solve:
$$
\begin{pmatrix}
\cos\theta & \sin\theta\\
\sin\theta & -\cos\theta
\end{pmatrix} \begin{pmatrix} a \\ b \end{pmatrix} = \begin{pmatrix} a \\ b \end{pmatrix}.
$$

This yields two simultaneous equations:
$$
\cos\theta \cdot a + \sin\theta \cdot b = a,
$$
$$
\sin\theta \cdot a - \cos\theta \cdot b = b.
$$
We rearrange the first equation:
$$
\cos\theta a + \sin\theta b = a,
$$
$$
(\cos\theta - 1)a + \sin\theta b = 0.
$$
From the second equation:
$$
\sin\theta a - \cos\theta b = b,
$$
$$
\sin\theta a - (\cos\theta + 1) b = 0.
$$

This can be written in matrix form as:
$$
\begin{pmatrix}
\cos\theta - 1 & \sin\theta \\
\sin\theta & -(\cos\theta + 1)
\end{pmatrix} \begin{pmatrix} a \\ b \end{pmatrix} = \begin{pmatrix} 0 \\ 0 \end{pmatrix}.
$$

To solve such a homogeneous system, we need the determinant of the matrix to be zero (which is usually checked while solving for the eigenvalues, but here we already know that an eigenvalue is $1$, so we need to solve for $a$ and $b$ such that the linear system is consistent):
$$
\begin{vmatrix}
\cos\theta - 1 & \sin\theta \\
\sin(theta) & -(\cos\theta + 1)
\end{vmatrix} = -(\cos^2\theta - 1) - \sin^2\theta.
$$

However, what we need here is a non-trivial solution for $a$ and $b$. Another way to solve for $a$ and $b$ is directly solving those two equations individually. From the first equation $(\cos\theta - 1)a + \sin\theta b = 0$, it follows that:
$$
\sin\theta b = (1 - \cos\theta)a,
$$
which implies,
$$
b = \frac{1 - \cos\theta}{\sin\theta} a,
$$
or using the identity $\frac{1 - \cos\theta}{\sin\theta}\,=\,\tan (\theta/2)$ for $\sin\theta \neq 0$ (another identity that works here is $\frac{1 - \cos\theta}{\sin\theta} = \tan\left(\frac{\theta}{2}\right)$),
$$
b = a \tan\left(\frac{\theta}{2}\right).
$$
Alternatively, one can check the second equation $\sin\theta a -(\cos\theta + 1) b = 0$, which implies,
$$
\sin\theta a = (\cos\theta + 1) b,
$$
thus,
$$
a = \frac{\cos\theta + 1}{\sin\theta} b,
$$
which is another valid expression. However, a more common identity here is $\frac{\sin\theta}{1 + \cos\theta} \,=\, \tan\left(\frac{\theta}{2}\right)$, so,
$$
a = \frac{b}{\tan(\theta/2)}.
$$
(This identity is derived from $\sin\theta = 2\sin\left(\frac{\theta}{2}\right)\cos\left(\frac{\theta}{2}\right)$ and $\cos\theta + 1 = 2\cos^2\left(\frac{\theta}{2}\right)$ such that $\frac{\sin\theta}{1 + \cos\theta} = \tan\frac{\theta}{2}$, implying that once $b$ is expressed in relation to $a$ such as $b = \tan\frac{\theta}{2}a$, the symmetric relation $a = \frac{b}{\tan(\theta/2)}$ should thus hold.)

To normalize the eigenvector $\binom{a}{b}$ such that $b = a \tan\frac{\theta}{2}$, let us assume $a = C$, thus $b = C \tan\frac{\theta}{2}$ such that the eigenvector could be written as:
$$
\begin{pmatrix} a \\ b \end{pmatrix} = C \begin{pmatrix} 1 \\ \tan\frac{\theta}{2} \end{pmatrix}.
$$
where $C$ is a normalization constant such that:
$$
|C|^2 \left[1 + \tan^2\frac{\theta}{2}\right] = 1.
$$
$$
\text{(Normalization condition implies } |a|^2 + |b|^2 = 1 \text{ for a normalized eigenvector)}.
$$
Since $1 + \tan^2\frac{\theta}{2} = \sec^2\frac{\theta}{2}$, it follows that:
$$
|C|^2 \sec^2\frac{\theta}{2} = 1,
$$
thus,
$$
|C| = |\cos\frac{\theta}{2}|.
$$
Hence, $C$ could be $\cos\frac{\theta}{2}$ (we can ignore the absolute value if we consider $C$ real and positive, which makes sense here because any phase factor $e^{i\phi}$ for $\cos\frac{\theta}{2}$ would disappear when normalizing the vector).

Thus, a normalized eigenvector corresponding to the eigenvalue $\frac{\hbar}{2}$ could be written as:
$$
\begin{pmatrix} a \\ b \end{pmatrix} = \cos\left(\frac{\theta}{2}\right) \begin{pmatrix} 1 \\ \tan\left(\frac{\theta}{2}\right) \end{pmatrix} = \begin{pmatrix} \cos\left(\frac{\theta}{2}\right) \\ \sin\left(\frac{\theta}{2}\right) \end{pmatrix}.
$$

To double check, another well-known expression for a spin-up eigenvector (spin aligned along the direction defined by the polar angles $\theta$ and $\phi$, where here $\phi = 0$ because the vector lies in the $x-z$ plane) for a spin-$\frac{1}{2}$ particle is:
$$
\begin{pmatrix} \cos\left(\frac{\theta}{2}\right) \\ e^{i\phi}\sin\left(\frac{\theta}{2}\right) \end{pmatrix}.
$$
However, here $\phi = 0$, so the expression becomes:
$$
\begin{pmatrix} \cos\left(\frac{\theta}{2}\right) \\ \sin\left(th\frac{\theta}{2}\right) \end{pmatrix}.
$$
Hence, this matches another well-know result for a spin-1/2 system where the spin is along an arbitrary direction $\vec{n}$ described by angles $\theta$ and $\phi$, except here we only need to use $\theta$ because the unit vector lies only in the $x$-$z$ plane (i.e., no $y$-component).

Thus, the normalized eigenvector can be verified directly by plugging it back into the initial eigenvalue problem:
$$
\vec{P} \cdot \vec{n} \begin{pmatrix} \cos\left(\frac{\theta}{2}\right) \\ \sin\left(\frac{\theta}{2}\right) \end{pmatrix} = \frac{\hbar}{2} \begin{pmatrix}
\cos\theta & \sin\theta\\
\sin\theta & - \cos\theta
\end{pmatrix} \begin{pmatrix} \cos\left(\frac{\theta}{2}\right) \\ \sin\left(\frac{\theta}{2}\right)\end{pmatrix}.
$$
$$
= \frac{\hbar}{2} \begin{pmatrix}
\cos\theta \cos\left(\frac{\theta}{2}\right) + \sin\theta \sin\left(\frac{\theta}{2}\right) \\
\sin\theta \cos\left(\frac{\theta}{2}\right) - \cos\theta \sin\left(\frac{\theta}{2}\right)
\end{pmatrix}.
$$
$$
= \frac{\hbar}{2} \begin{pmatrix}
\cos\theta \cos\left(\frac{\theta}{2}\right) + \sin\theta \sin\left(\frac{\theta}{2}\right) \text{ (which is $\cos\left(\theta - \frac{\theta}{2}\right) = \cos\frac{\theta}{2}$)} \\
\sin\theta \cos\left(\frac{\theta}{2}\right) - cos\theta \sin\left(\frac{\theta}{2}\right) \text{ (which is $\sin\left(\theta - \frac{\theta}{2}\right) = \sin\frac{\theta}{2}$)}
\end{pmatrix}.
$$
$$
= \frac{\}{2} \begin{pmatrix}
\cos\left(\frac{\theta}{2}\right) \\
\sin\left(\frac{\theta}{2}\right)
\end{pmatrix}.
$$
which confirms that the normalized eigenvector for the eigenvalue $+\frac{\hbar}{2}$ is:
$$
\begin{pmatrix} \cos\left(\frac{\theta}{2}\right) \\ \sin\left(\frac{\theta}{2}\right) \end{pmatrix}.
$$
This normalized eigenvector is indeed an eigenvector of $\vec{P} \cdot \vec{n}$ corresponding to the eigenvalue $+\frac{\hbar}{2}$.

### Conclusion:
The normalized eigenvector corresponding to eigenvalue $+\frac{\hbar}{2}$ can be written explicitly as:
$$
\begin{pmatrix} \cos(\theta/2) \\
\sin(\theta/2)
\end{pmatrix}.
$$
So, listing the elements of the normalized eigenvector explicitly we have:
$$
\text{Elements are: }\cos\frac{\theta}{2} \textrm{ and } \sin\frac{\theta}{2}.
$$

However, an explicit alternative representation could confirm the result by directly solving the matrix $ \vec{P} \cdot \vec{n}$ eigenvalues explicitly. However, the task already provided an eigenvalue and we verified what the normalized eigenvector should be, making us confident that:
$$
\vec{v} = \begin{pmatrix} \cos\frac{\theta}{2} \\ \sin\frac{\theta}{2} \end{pmatrix}.
$$

So, the answer is:
$$
\begin{pmatrix} \cos(\theta/2) \\ \sin(\theta/2) \end{pmatrix}.
$$
Although another possible context should be validated by diagonalizing $\vec{P} \cdot \vec{n}$ explicitly but the question already makes an eigenvalue assumption such that $\vec{v}$ aligns with the spin resolved by $+\frac{\hbar}{2}$.

However, to make sure that there is no misunderstanding, let us directly verify the eigenvalues of the matrix $A$:
$$
A = \begin{pmatrix}
\cos\theta & \sin\theta \\
\sin\theta & -\cos\theta
\end{pmatrix}.
$$
The eigenvalue equation $|\begin{pmatrix}
\cos\theta - \lambda & \sin\theta \\
\sin\theta & -\cos\theta - \lambda
\end{pmatrix}| = 0$ yields:
$$
(\cos\theta - \lambda)(-\cos\theta - \lambda) - \sin^2\theta = 0.
$$
$$
\lambda^2 - \cos^2\theta - \sin^2\theta = 0,
$$
$$
\lambda^2 - (\sin^2\theta + \cos^2\theta) = 0,
$$
$$
\lambda^2 - 1 = 0,
$$
$$
\lambda = \pm 1.
$$
This confirms that the eigenvalues of $A$ are $\pm1$, so the eigenvalues of $ \vec{P} \cdot \vec{n} = \frac{\hbar}{2}A$ are $\pm\frac{\hbar}{2}$ which confirms that an eigenvalue $+\frac{\hbar}{2}$ does indeed exist.

To make everything perfectly clear let us verify what the eigenvalues $1$ and $-1$ correspond to for the matrix $A$ itself:

For $\lambda = 1$:
$$
\begin{pmatrix}
\cos\theta & \sin\theta \\
\sin\theta & -\cos\theta
\end{pmatrix} \begin{pmatrix} u_1 \\ u_2 \end{pmatrix} = \begin{pmatrix} u_1 \\ u_2 \end{pmatrix}.
$$
which we already solved previously (which led us to the eigenvector $\begin{pmatrix} \cos\left(\frac{\theta}{2}\right) \\ \sin\left(\frac{\theta}{2}\right) \end{pmatrix}$).

For $\lambda = -1$:
$$
\begin{pmatrix}
cos\theta & \sin\theta \\
\sin\theta & -\cos\theta
\end{pmatrix} \begin{pmatrix} u_1 \\ u_2 \end{pmatrix} = - \begin{pmatrix} u_1 \\ u_2 \end{pmatrix}.
$$
which leads to the system of equations:
$$
\cos\theta u_1 + sin\theta u_2 = -u_1.
$$
$$
sin\theta u_1 - \cos\theta u_2 = -u_2.
$$
$$
\Rightarrow (\cos\theta + 1)u_1 + \sin\theta u_2 = 0,
$$
$$
\sin\theta u_1 + (1 - cos\theta) u_2 = 0.
$$
From the first equation:
$$
\sin\theta u_2 = -(\cos\theta + 1)u_1.
$$
$$
u_2 = -\frac{\cos\theta + 1}{\sin\theta}u_1 = -\frac{1 + \cos\theta}{\sin\theta} u_1.
$$
Since $\frac{1 + \cos\theta}{\sin\theta} = \cot\frac{\theta}{2}$,
$$
u_2 = -u_1 \cot\left(\frac{\theta}{2}\right).
$$
Normalizing such that $u_1 = C$ and $u_2 = -C \cot\left(\frac{\theta}{2}\right)$:
$$
\binom{u_1}{u_2} = C \binom{1}{-\cot\left(\frac{\theta}{2}/\right)}.
$$
Normalizing this:
$$
1 = |C|^2\left(1 + \cot^2\left(\frac{\theta}{2}\right)\right).
$$
$$
1 = |C|^2\csc^2\left(\frac{\theta}{2}\right).
$$
$$
|C| = \sin\left(\frac{\theta}{2}\right).
$$
Therefore, another normalized eigenvector (for the eigenvalue $-\frac{\hbar}{2}$ in the operator $\vec{P} \cdot \vec{n}$):
$$
\binom{u_1}{u_2} = \sin\left(\frac{\theta}{2}\right) \binom{1}{-\cot\left(\frac{\theta}{2}\right)} = \binom{\sin\left(\frac{\theta}{2}\right)}{ -\sin\left(\frac{\theta}{2}\right)\cot\left(\frac{\theta}{2}\right)}.
$$
$$
= \binom{\sin\left(\frac{\theta}{2}\right)}{-\cos\left(\frac{\theta{J}{2}\right)}.
$$
Thus if $\

---

