# Original Question

An electron is in the spin state (3i, 4). Find the expectation value of its spin along y-direction, S_y.
Note: \sigma_y (in latex format) is: 
\begin{pmatrix}
0 & -i \\
i & 0
\end{pmatrix}

---

# DeepSeek response (via openrouter)

\boxed{-\frac{12\hbar}{25}}

---

# DeepSeek reasoning (via openrouter)

To solve for the expectation value of the spin along the $y$-direction $S_y$ for an electron in the spin state represented by the spinor $\chi = \binom{3i}{4}$, we need to recall that the spin operator for the $y$-direction is given by:
$$
S_y = \frac{\hbar}{2} \sigma_y,
$$
where:
$$
\sigma_y = \begin{pmatrix}
0 & -i \\
i & 0
\end{pmatrix}.
$$
The spin state is given as $\binom{3i}{4}$, which can be written as:
$$
\chi = \begin{pmatrix} 3i \\ 4 \end{pmatrix}.
$$
The usual form of a spin state for a spin-1/2 particle (such as an electron) is:
$$
\chi = \begin{pmatrix} a \\ b \end{pmatrix},
$$
where $a$ and $b$ are complex numbers. Here, $a=3i$ and $b=4$.

The question is to find the expectation value of the spin operator $S_y$. Recall that the expectation value of an operator $A$ in a state $\chi$ is given by:
$$
\langle A \rangle = \frac{\langle \chi | A | \chi \rangle}{\langle \chi | \chi \rangle}.
$$
However, if the state $\chi$ is normalized such that $\langle\chi | \chi \rangle = 1$, the expectation value can be computed as:
$$
\langle A \rangle = \langle \chi | A | \chi \rangle.
$$
However, given the question here, one should first verify if the given spin state is normalized. Normalization requires:
$$
\langle \chi | \chi \rangle = |\chi|^2 = |3i|^2 + |4|^2 = |3i|^2 + 16.
$$
Calculating $|-3i|^2$:
$$
|3i|^2 = |3i \cdot 3i^*| = (3i) \cdot (-3i) = 9,
$$
thus:
$$
\langle \chi | \chi \rangle = |3i|^2 + 16 = 9 + 16 = 25.
$$
(Alternatively, directly compute $|3i|^2 = (3i)(3i)^* = (3i)(-3i) = 9$.)

Since the state is evidently not normalized (since $\binom{3i}{4}$ has inner product $25$), let us first denote the normalization constant such that the normalized state is:
$$
\chi_{\text{norm}} = \frac{1}{\sqrt{25}} \begin{pmatrix} 3i \\ 4 \end{pmatrix} = \frac{1}{5} \begin{pmatrix} 3i \\ 4 \end{pmatrix} = \begin{pmatrix} \dfrac{3i}{5} \\ \dfrac{4}{5} \end{pmatrix}.
$$
But let us first verify the normalized state explicitly:
$$
\chi_{\text{norm}} = \frac{1}{5} \begin{pmatrix} 3i \\ 4 \end{pmatrix}.
$$
We need to find the expectation value for $S_y$:
$$
\langle S_y \rangle = \langle \chi_{\text{norm}} \mid S_y \mid \chi_{\text{norm}} \rangle.
$$
However, $S_y = \frac{\hbar}{2} \sigma_y$, so:
$$
\langle S_y \rangle = \langle \chi_{\text{norm}} \mid \frac{\hbar}{2} \sigma_y \mid \chi_{\text{norm}} \rangle = \frac{\hbar}{2} \langle \chi_{\text{norm}} \mid \sigma_y \mid \chi_{\text{norm}} \rangle.
$$
We need to evaluate $\langle \chi_{\text{norm}} | \sigma_y | \chi_{\text{norm}} \rangle$. For this, first recall that:
$$
|\chi_{\text{norm}} \rangle = \frac{1}{5} \begin{pmatrix} 3i \\ 4 \end{pmatrix}.
$$
Then the bra vector (complex conjugate transpose of the ket vector) is:
$$
\langle \chi_{\text{norm}} | = \frac{1}{5} \begin{pmatrix} 3i \\ 4 \end{pmatrix}^\dagger = \frac{1}{5} \begin{pmatrix} (3i)^* & 4^* \end{pmatrix} = \frac{1}{5} \begin{pmatrix} -3i & 4 \end{pmatrix}.
$$
Note that the bra vector is a row vector where $a^*$ and $b^*$ should be the entries such that:
$$
\begin{pmatrix}a\\ b\end{pmatrix}^\dagger = (a^*\, \, \, b^*).
$$
Once we have the bra and ket vectors, we need to apply the $\sigma_y$ matrix to the ket vector $|\chi_{\text{norm}}\rangle$:
$$
\sigma_y |\chi_{\text{norm}}\rangle = \begin{pmatrix} 0 & -i \\ i & 0 \end{pmatrix} \left(\frac{1}{5} \begin{pmatrix} 3i \\ 4 \end{pmatrix}\right) = \frac{1}{5} \begin{pmatrix} 0 & -i \\ i & 0 \end{pmatrix} \begin{pmatrix} 3i \\ 4 \end{pmatrix}.
$$
Using matrix multiplication:
$$
\frac{1}{5}\begin{pmatrix} 0 & -i \\ i & 0 \end{pmatrix} \begin{pmatrix} 3i \\ 4 \end{pmatrix} = \frac{1}{5} \begin{pmatrix} 0 \cdot 3i + (-i) \cdot 4 \\ i \cdot 3i + 0 \cdot 4 \end{pmatrix} = \frac{1}{5} \begin{pmatrix} -4i \\ i \cdot 3i \ \end{pmatrix}.
$$
Since $i \cdot 3i = 3i^2 = -3$:
$$
\frac{1}{5} \begin{pmatrix} -4i \\ -3 \end{pmatrix}.
$$
So now, we need to compute the inner product $\langle \chi_{\text{norm}} \mid \sigma_y \mid \chi_{\text{norm}} \rangle$:
$$
\langle \chi_{\text{norm}} \mid \sigma_y \mid \chi_{\text{norm}} \rangle = \left(\frac{1}{5} \begin{pmatrix} -3i & 4 \end{pmatrix}\right) \left(\frac{1}{5} \begin{pmatrix} -4i \\ -3 \end{pmatrix}\right).
$$
Again pulling constants outside:
$$
= \left(\frac{1}{5}\right) \left(\frac{1}{5}\right) \begin{pmatrix} -3i & 4 \end{pmatrix} \begin{pmatrix} -4i \\ -3 \end{pmatrix} = \frac{1}{25} \left[(-3i)(-4i) + 4 \cdot (-3)\right].
$$
Calculating the inner product:
$$
(-3i)(-4i) = (3i)(4i) = 12i^2 = -12,
$$
$$
4 \times (-3) = -12,
$$
$$
\begin{pmatrix} -3i & 4 \end{pmatrix} \begin{pmatrix} -4i \\ -3 \end{pmatrix} = -12 - 12 = -24,
$$
So:
$$
\langle \chi_{\text{norm}} | \sigma_y | \chi_{\text{norm}} \rangle = \frac{1}{25} \times (-24) = -\frac{24}{25}.
$$
To find the expectation value of $S_y$:
$$
\langle S_y \rangle = \frac{\hbar}{2} \langle \chi_{\text{norm}} \mid \sigma_y \mid \chi_{\text{norm}} \rangle = \frac{\hbar}{2} \times \left(-\frac{24}{25}\right) = -\frac{12}{25}\hbar.
$$

So, the expectation value of $S_y$ is:
$$
\boxed{-\frac{12\hbar}{25}}.
$$

We should double-check all calculations thoroughly:
To verify normalization again:
$$
\left|\binom{a}{b}\right| =\sqrt{|a|^2 + |b|^2} \text{ where } |a|^2 + |b|^2 = 1\text{ (for state normalization)}.
$$
Normalized state check:
$$
\chi_{\text{norm}} = \binom{\dfrac{3i}{5}}{\dfrac{4}{5}}.
$$
Double-check normalization condition:
$$
\left|\binom{\frac{3i}{5}}{\frac{4}{5}}\right|^2 = \left|\frac{3i}{5}\right)^2 + \left(\frac{4}{5}\right|^2 = \left(\frac{3i}{5} \times \frac{-3i}{5}\right) + \left(\frac{16}{25}\right) = \frac{9i \cdot (-i)}{25} + \frac{16}{25} = \frac{9}{25} + \frac{16}{25} = 1.
$$

So, the state is indeed normalized correctly here where $\binom{\frac{3i}{5}}{\frac{4}{5}}$ is the normalized state. 

This leads us to make a double verification again for the matrix multiplication operations independently:
$$
\sigma_y \binom{a}{b} = \binom{0 \cdot a - ib}{ia + 0 \cdot b} = \binom{- ib}{ia}.
$$
For $a=3i$ and $b=4$, if directly using the original $3i$ and $binom{3i}{4}$ as a state (ignoring the normalization until the last step):
$$
\sigma_y \binom{3i}{4} = \binom{0 \cdot 3i - i \cdot 4}{i \cdot 3i + 0 \cdot 4} = \binom{-4i}{-3}.
$$
This part seems okay so far. 

Next, taking inner product with the original state (not normalized yet):
$$
\binom{3i}{4}^\dagger = (-3i, 4).
$$
So:
$$
\langle \chi | S_y | \chi \rangle = \langle \binom{3i}{4} | S_y | \binom{3i}{4} \rangle = -\frac{3i}{2}(-4i) + 4 \times -3,
$$
We need to make another round of verification here:
$$
\langle S_y \rangle_\text{unnormalized} = (-3i, 4) \cdot \frac{\hbar}{2} \binom{0}{-i} \binom{i}{0} \binom{3i}{4} = \frac{\hbar}{2}(-3i, 4) \binom{-4i}{-3} = \frac{\hbar}{2} \left((-3i, 4) \binom{-4i}{-3}\right).
$$
$$
= \frac{\hbar}{2}[(-3i) \times (-4i) + 4 \times (-3)] = \frac{\hbar}{2}[-(3i) \times (4i) - 12] = \frac{\hbar}{2}[-12i^2 - 12] = \frac{\hbar}{2}[12 - 12] \text{ (incorrect step here)}.
$$
The $-12i^2 + 4 \times (-3) = 12-12 = 0$ seems off. Let us make a clear step-by-step verification again.

Update previous line-by-line computation correctly:
First compute:
$$
(-3i, 4) \binom{-4i}{:-3} = ((-3i) \times (-4i)) + 4 \times (-3) = (-3i) \times (-4i) + 4 \times (-3) = 12 i^2 - 12.
$$
Since $i^2 = -1$,
$$
=12(-1) - 12 = -12 - 12 = -24.
$$

However, it appears that the small error previously overlooked here needs a cross-check. Another way around this is by directly using the normalized state:

Let us remind ourselves what the normalized state $|\chi_{\text{norm}}\rangle$ looks like:
$$
|\chi _{\text{norm}}\rangle = \binom{\frac{3i}{5}}{\frac{4}{5}} = \begin{pmatrix} \frac{3i}{5} \\ \frac{4}{5} \end{pmatrix}.
$$
Similarly:
Bra vector:
$$
\langle \chi_{\text{norm}} | = \langle \left(\frac{3i}{5}, \frac{4}{5}\right) | = \left(\frac{-3i}{5}, \frac{4}{5}\right).
$$
Acting $\sigma_y$ on $|\chi_{\text{norm}}\rangle$:
$$
\sigma_y |\chi_{\text{norm}}\rangle = \binom{0 \cdot \frac{3i}{5} - i \cdot \frac{4}{5}}{i \cdot \frac{3i}{5} + 0 \cdot \\fourth{5}} = \binom{\frac{-4i}{5}}{\frac{i \cdot 3i}{5}} = \binom{\frac{-4i}{5}}{\frac{-3}{5}} = \binom{\frac{-4i}{5}}{\frac{-3}{5}} = \binom{\frac{-4i}{5}}{\frac{-3}{5}}.
$$
Taking the inner product:
$$
\langle \chi_{\text{norm}}|\sigma_y|\chi_{\text{norm}}\rangle = \left(\frac{-3i}{5}\,\, \frac{4}{5}\right)\binom{-4i/5}{-3/5} = \left(\frac{-3i}{5}\right) \times \left(\frac{-4i}{5}\right) + \left(\frac{4}{5}\right) \times \left(\frac{-3}{5}). 
$$

Again, first compute individual products:
$$
\left(\frac{-3i}{5}\right) \times \left(\frac{-4i}{5} \right)= \frac{12i^2}{25} = \frac{12 \times (-1)}{25} = \frac{-12}{25}.
$$
$$
\left(\frac{4}{5}\right) \times \left(\frac{-3}{5}\right) = \frac{-12}{25}.
$$
Combine both terms together gives:
$$
\langle \chi_{\text{norm}}|\sigma_y|\chi_{\text{norm}}\rangle = \frac{-12}{25} +\frac{-12}{25} = -\frac{24}{25}.
$$

Result derived from $S_y = \frac{\hbar}{2} \sigma_y$:
$$
\langle S_y\rangle = \frac{\hbar}{2} \langle \chi_{\text{norm}}| \sigma_y | \chi_{\text{norm}} \rangle = \frac{\hbar}{2} \times \left(-\frac{24}{25}\right) = -\frac{24}{25} \times \frac{\hbar}{2} = -\frac{24}{50} \hbar = -\frac{12}{25}\hbar.
$$
That seems to agree uniformly.

You can validate alternative normalizations another way for back-checking. For any state $|\chi\rangle$, the expectation value of an operator $S_y$ is given by:
$$
\langle S_y \rangle = \frac{\langle\chi | S_y | \chi\rangle}{\langle \chi | \chi \rangle}.
$$
Thus, if we assert the state $|\chi\rangle=\binom{3i}{4}$ which isn't normalized where:
$$
|\chi\rangle = \binom{3i}{4}.
$$
The normalizing denominator is $\langle \chi | \chi \rangle = 25$:
$$
\langle S_y \rangle = \frac{\binom{-3i \, 4} \frac{\hbar}{2} \binom{0\, -i}{i \, \, 0} \binom{3i}{4}}{\binom{-3i \, 4} \binom{3i}{4}}.
$$
Calculating separately:
$$
\binom{-3i \, 4} \frac{\hbar}{2} \binom{0\, -i}{i \, 0} \binom{3i}{4} \\
= \binom{-3i \, 4} \frac{\hbar}{2} \binom{0 \cdot 3i - i \cdot 4}{i \cdot 3i \phantom{0} + 0 \cdot 4}\\ 
= \binom{-3i \, 4} \frac{\hbar}{2} \binom{-4i}{-3} = \frac{\hbar}{2} \left[(-3i) \cdot(-4i) + 4 \cdot(-3)\right]\\
= \frac{\hbar}{2}[( -3i)\cdot(-4i) + 4 \cdot (-3)]\\
= \frac{\hbar}{2}( 12i^2 - 12) = \frac{\hbar}{2}(-12 - 12) = \frac{\hbar}{2}(-24) = -12 \hbar.
$$
As for the normalizing denominator:
$$
\binom{-3i\quad 4}\binom{3i}{4} ={-3i \times 3i + 4 \times 4}.
$$
$$
{-3i \times 3i} = -9i^2 = -9(-1) = 9,
$$
Thus:
$$
{-elastic \times 3i = 4} + 4 \times 4 = 9 + 16 = 25.
$$
Hence:
$$
\langle S_y \rangle = \frac{-12\hbar}{25},
$$
which is what we found previously when we explicitly dealt with the normalized spinor $\binom{3i/5}{4/5}$.

So this answer supports the previous one. Thus ${\dfrac{-12\hbar}{25}}$ appears to be the consensus.


---

