# Original Question

 Consider a 1-dimensional relativistic harmonic oscillator with mass $m$ and maximum amplitude $A$ obeying Hook's law ($F=-kx$). What is the maximum speed  $v_max$ of the mass? The speed of light is $c$.

---

# DeepSeek response (via openrouter)



---

# DeepSeek reasoning (via openrouter)

To solve for the maximum speed $v_{\text{max}}$ of a 1-dimensional relativistic harmonic oscillator with mass $m$ and a restoring force given by Hooke's law $F = -kx$, where $k$ is the spring constant and $A$ is the maximum amplitude, we need to make some adjustments to the usual non-relativistic treatment.

The force $F = -kx$ leads to a potential energy $U(x)$ such that:
$$
F = -\frac{dU}{dx} = -kx.
$$
Thus, the potential energy $U(x)$ can be found by integrating:
$$
U(x) = \int_0^x kx'\, dx' = \frac{1}{2}kx^2,
$$
where we have set the constant of integration such that $U(0) = 0$.

However, in a relativistic context, the total energy $E$ of a particle with rest mass $m$ is given by:
$$
E = \gamma mc^2,
$$
where $\gamma$ is the Lorentz factor defined as:
$$
\gamma = \frac{1}{\sqrt{1 - \frac{v^2}{c^2}}}.
$$
The total energy can also be split into the rest energy $mc^2$ and the kinetic energy $T$ such that:
$$
E = mc^2 + T.
$$
However, a more common way to express the total energy is:
$$
E = \sqrt{(mc^2)^2 + (pc)^2},
$$
where $p$ is the relativistic momentum given by:
$$
p = \gamma mv.
$$
However, another way to express the total energy is:
$$
E = \gamma mc^2 = mc^2 + T,
$$
where $T$ is the kinetic energy defined as:
$$
T = (\gamma - 1)mc^2.
$$
However, another well-known expression for the total energy is:
$$
E = mc^2 + T = mc^2 + U(x) + K,
$$
where $K$ is the "kinetic energy" in the usual sense (which should be $T$ here). However, what we need here is a conservation of energy equation where the total energy includes the rest energy $mc^2$, the potential energy $U(x)$, and the "total energy" (which includes rest energy and kinetic energy).

The total energy $E_{\text{tot}}$ can be written as:
$$
E_{\text{tot}} = \gamma mc^2 + U(x) = \gamma mc^2 + \frac{1}{2}kx^2.
$$
However, this seems a bit off because the total energy should be a constant sum of the rest energy, the potential energy, and the "relativistic energy" (which already includes the rest energy). A more appropriate way to express the total energy might be:
$$
E_{\text{tot}} = \gamma mc^2,
$$
where the total energy should be conserved such that:
$$
\gamma mc^2 = \text{constant}.
$$
However, a more common way to express the total energy in a system where there is a potential energy $U(x)$ is:
$$
E_{\text{tot}} = \gamma mc^2 + U(x) = \gamma mc^2 + \frac{1}{2}kx^2.
$$
However, a more standard way to write the total energy for a relativistic particle in a potential $U(x)$ is:
$$
E_{\text{tot}} = \sqrt{(mc^2)^2 + (pc)^2} + U(x).
$$
However, a more common form used in relativistic mechanics is:
$$
E_{\text{tot}} = \sqrt{(mc^2)^2 + (pc)^2} = \sqrt{(mc^2)^2 + (m\gamma v c)^2} = \gamma mc^2.
$$
This makes us realize that the total energy should be:
$$
E_{\text{tot}} = \gamma mc^2 + \frac{1}{2}kx^2.
$$
However, a more "correct" way to write the total energy might be:
$$
E_{\text{tot}} = \gamma mc^2 = \text{constant}.
$$
However, what we need here is a "Hamiltonian" for a relativistic particle in a potential $U(x)$ such that:
$$
\mathcal{H} = \sqrt{(mc^2)^2 + (pc)^2} + U(x).
$$
However, a more "correct" Hamiltonian for a relativistic harmonic oscillator should be:
$$
\mathcal{H} = \sqrt{(mc^2)^2 + (pc)^2} + \frac{1}{2}kx^2.
$$
However, a more "intuitive" way to solve for the total energy might be:
$$
E_{\text{tot}} = \text{kinetic energy} + \text{potential energy} + \text{rest energy}.
$$
However, the "kinetic energy" here should be the relativistic kinetic energy $T = (\gamma - 1)mc^2$, so:
$$
E_{\text{tot}} = (\gamma - 1)mc^2 + \frac{1}{2}kx^2 + mc^2 = \gamma mc^2 + \frac{1}{2}kx^2.
$$
However, this seems a bit redundant because the total energy should be a constant sum. Another way to make sure that the total energy is conserved is:
$$
E_{\text{tot}} = \gamma mc^2 + \frac{1}{2}kx^2.
$$
However, a more "standard" way to write the total energy is:
$$
E_{\text{tot}} = \gamma mc^2.
$$
However, the part that makes sense here is that the total energy should be conserved. Thus, the total energy at any point $x$ should be equal to the total energy at the maximum amplitude $A$ where $x = A$ and $v = 0$ (since $A$ is the point where the oscillator reverses direction, so the velocity is zero there).

At $x = A$, the velocity is zero (i.e., $v = 0$), so $\gamma = 1$:
$$
E_{\text{tot}} = mc^2 + \frac{1}{2}kA^2.
$$
This is because:
$$
\gamma = \frac{1}{\sqrt{1 - \frac{v^2}{c^2}}} \text{ where } v = 0 \text{ so } \gamma = 1.
$$
Thus, the total energy at $x = A$ is:
$$
E_{\text{tot}} = mc^2 + \frac{1}{2}kA^2.
$$
At any other point $x$ where the velocity is $v$, the total energy should be:
$$
E_{\text{tot}} = \gamma mc^2 + \frac{1}{2}kx^2.
$$
However, this seems a bit off. Another part of the total energy should be:
$$
E_{\text{tot}} = \gamma mc^2.
$$
However, what we need is a consistent way to express the total energy. Another way to make sure that the total energy is conserved is:
$$
mc^2 + \frac{1}{2}kA^2 = \gamma mc^2 + \frac{1}{2}kx^2.
$$
However, another part of the total energy should be:
$$
mc^2 + \frac{1}{2}kA^2 = \gamma mc^2.
$$
However, the first part seems a bit more logical because it makes sense that the total energy should be the sum of the rest energy, the potential energy, and the kinetic energy (which is already included in the $\gamma mc^2$ term).

However, a more "correct" way to solve for the total energy might be:
$$
E_{\text{tot}} = \sqrt{(mc^2)^2 + (pc)^2} + \frac{1}{2}kx^2.
$$
However, the total energy should be a constant. Thus, at $x = A$ where $v = 0$, $p = 0$:
$$
E_{\text{tot}} = \sqrt{(mc^2)^2} + \frac{1}{2}kA^2 = mc^2 + \frac{1}{2}kA^2.
$$
At any other point $x$ where $v \neq 0$:
$$
E_{\text{tot}} = \sqrt{(mc^2)^2 + (pc)^2} + \frac{1}{2}kx^2.
$$
However, the total energy should be the same:
$$
mc^2 + \frac{1}{2}kA^2 = \sqrt{(mc^2)^2 + (pc)^2} + \frac{1}{2}kx^2.
$$
However, the question is asking for the maximum speed $v_{\text{max}}$, which should occur when the potential energy is at a minimum (i.e., when $x = 0$). At $x = 0$, the potential energy is:
$$
U(0) = \frac{1}{2}k \cdot 0^2 = 0.
$$
So, the total energy at $x = 0$ should be:
$$
mc^2 + \frac{1}{2}kA^2 = \sqrt{(mc^2)^2 + (pc)^2} + \frac{1}{2}k \cdot 0^2.
$$
$$
mc^2 + \frac{1}{2}kA^2 = \sqrt{(mc^2)^2 + (pc)^2}.
$$
$$
mc^2 + \frac{1}{2}kA^2 = \sqrt{(mc^2)^2 + (\gamma mv c)^2}.
$$
However, $p = \gamma mv$, so:
$$
mc^2 + \frac{1}{2}kA^2 = \sqrt{(mc^2)^2 + (\gamma mvc)^2} = \sqrt{(mc^2)^2 + \gamma^2 m^2 v^2 c^2}.
$$
However, since $\gamma = \frac{1}{\sqrt{1 - \frac{v^2}{c^2}}}$, it follows that:
$$
\gamma^2 = \frac{1}{1 - \frac{v^2}{c^2}}.
$$
Thus:
$$
mc^2 + \frac{1}{2}kA^2 = \sqrt{(mc^2)^2 + \frac{m^2 v^2 c^2}{1 - \frac{v^2}{c^2}}}.
$$
$$
mc^2 + \frac{1}{2}kA^2 = \sqrt{m^2c^4 + \frac{m^2 v^2 c^2}{1 - \frac{v^2}{c^2}}}.
$$
$$
mc^2 + \frac{1}{2}kA^2 = mc^2 \sqrt{1 + \frac{\frac{m^2 v^2 c^2}{1 - \frac{v^2}{c^2}}}{m^2 c^4}}.
$$
$$
mc^2 + \frac{1}{2}kA^2 = mc^2 \sqrt{1 + \frac{v^2}{c^2 - v^2}}.
$$
$$
mc^2 + \frac{1}{2}kA^2 = mc^2 \sqrt{\frac{c^2 - v^2 + v^2}{c^2 - v^2}}.
$$
$$
mc^2 + \frac{1}{2}kA^2 = mc^2 \sqrt{\frac{c^2}{c^2 - v^2}}.
$$
$$
mc^2 + \frac{1}{2}kA^2 = mc^2 \cdot \frac{c}{\sqrt{c^2 - v^2}}.
$$
$$
mc^2 + \frac{1}{2}kA^2 = \frac{mc^3}{\sqrt{c^2 - v^2}}.
$$
$$
mc^2 + \frac{1}{2}kA^2 = \frac{mc^3}{c\sqrt{1 - \frac{v^2}{c^2}}}.
$$
$$
mc^2 + \frac{1}{2}kA^2 = \frac{mc^2}{\sqrt{1 - \frac{v^2}{c^2}}}.
$$
$$
mc^2 + \frac{1}{2}kA^2 = \gamma mc^2.
$$
This makes us realize that the total energy should be:
$$
\gamma mc^2 = mc^2 + \frac{1}{2}kA^2.
$$
This makes sense because the total energy should be a constant sum of the rest energy $mc^2$, the potential energy (which is $\frac{1}{2}kA^2$ when $x = A$), and the kinetic energy (which is already included in the $\gamma mc^2$ term where $\gamma mc^2 = mc^2 + T$ where $T$ is the kinetic energy).

To find the maximum speed $v_{\text{max}}$, which should occur when $x = 0$ (since the potential energy is zero there and thus all the energy should be in the form of kinetic energy and rest energy), we need to solve for $v$ when $x = 0$:
$$
\gamma mc^2 = mc^2 + \frac{1}{2}kA^2.
$$
$$
\gamma = \frac{mc^2 + \frac{1}{2}kA^2}{mc^2} = 1 + \frac{kA^2}{2mc^2}.
$$
$$
\gamma = 1 + \frac{kA^2}{2mc^2}.
$$
Recall that:
$$
\gamma = \frac{1}{\sqrt{1 - \frac{v^2}{c^2}}}.
$$
So:
$$
1 + \frac{kA^2}{2mc^2} = \frac{1}{\sqrt{1 - \frac{v^2}{c^2}}}.
$$
$$
\sqrt{1 - \frac{v^2}{c^2}} = \frac{1}{1 + \frac{kA^2}{2mc^2}}.
$$
$$
1 - \frac{v^2}{c^2} = \left(\frac{1}{1 + \frac{kA^2}{2mc^2}}\right)^2.
$$
$$
1 - \frac{v^2}{c^2} = \left(\frac{2mc^2}{2mc^2 + kA^2}\right)^2.
$$
$$
1 - \frac{v^2}{c^2} = \left(\frac{2mc^2}{2mc^2 + kA^2}\right)^2.
$$
$$
\frac{v^2}{c^2} = 1 - \left(\frac{2mc^2}{2mc^2 + kA^2}\right)^2.
$$
$$
\frac{v^2}{c^2} = 1 - \left(\frac{4m^2c^4}{(2mc^2 + kA^2)^2}\right).
$$
$$
\frac{v^2}{c^2} = \frac{(2mc^2 + kA^2)^2 - 4m^2c^4}{(2mc^2 + kA^2)^2}.
$$
$$
\frac{v^2}{c^2} = \frac{(4m^2c^4 + 4mc^2kA^2 + k^2A^4) - 4m^2c^4}{(2mc^2 + kA^2)^2}.
$$
$$
\frac{v^2}{c^2} = \frac{4mc^2kA^2 + k^2A^4}{(2mc^2 + kA^2)^2}.
$$
$$
\frac{v^2}{c^2} = \frac{kA^2(4mc^2 + kA^2)}{(2mc^2 + kA^2)^2}.
$$
$$
v^2 = \frac{c^2kA^2(4mc^2 + kA^2)}{(2mc^2 + kA^2)^2}.
$$
$$
v^2 = \frac{c^2kA^2(4mc^2 + kA^2)}{(2mc^2 + kA^2)^2}.
$$
$$
v = c\sqrt{\frac{kA^2(4mc^2 + kA^2)}{(2mc^2 + kA^2)^2}}.
$$
$$
v = c\sqrt{\frac{kA^2(4mc^2 + kA^2)}{(2mc^2 + kA^2)^2}}.
$$
$$
v = c\sqrt{\frac{kA^2(4mc^2 + kA^2)}{4m^2c^4 + 4mc^2kA^2 + k^2A^4}}.
$$
$$
v = c\sqrt{\frac{kA^2(4mc^2 + kA^2)}{(4mc^2 + kA^2)mc^2 + kA^2(2mc^2 + kA^2)}}.
$$
However, a more "simplified" form might be:
$$
v = c\sqrt{\frac{kA^2(4mc^2 + kA^2)}{(2mc^2 + kA^2)^2}}.
$$
$$
v = c \cdot \frac{A\sqrt{k(4mc^2 + kA^2)}}{2mc^2 + kA^2}.
$$
$$
v = \frac{Ac\sqrt{k(4mc^2 + kA^2)}}{2mc^2 + kA^2}.
$$
However, a more "intuitive" way to solve for $v_{\text{max}}$ might be to solve for $v$ explicitly from the energy conservation equation:
$$
mc^2 + \frac{1}{2}kA^2 = \gamma mc^2.
$$
$$
\frac{1}{2}kA^2 = (\gamma - 1)mc^2.
$$
$$
\frac{kA^2}{2mc^2} = \gamma - 1.
$$
$$
\gamma = 1 + \frac{kA^2}{2mc^2}.
$$
$$
\frac{1}{\sqrt{1 - \frac{v^2}{c^2}}} = 1 + \frac{kA^2}{2mc^2}.
$$
$$
1 - \frac{v^2}{c^2} = \left(1 + \frac{kA^2}{2mc^2}\right)^{-2}.
$$
$$
\frac{v^2}{c^2} = 1 - \left(1 + \frac{kA^2}{2mc^2}\right)^{-2}.
$$
$$
v_{\text{max}} = c\sqrt{1 - \left(1 + \frac{kA^2}{2mc^2}\right)^{-2}}.
$$
This is a valid expression for $v_{\text{max}}$, which is the answer. However, we need to verify that this makes sense in the non-relativistic limit where $kA^2 \ll 2mc^2$. 

#### Non-relativistic limit check:
In the non-relativistic

---

