# Original Question

The state of a system at time t is given by the column matrix having elements (-1, 2, 1), and the operators of two observables P and Q of the system are represented by two square matrices. The matrix corresponding to operator P has the elements in first row as (0, 1/ \sqrt{2}, 0), elements in the second row as (1/ \sqrt{2}, 0, 1/ \sqrt{2}) and that in third row as (0, 1/ \sqrt{2}, 0). The matrix operator for Q is represented by the square matrix having elements in the first row as (1, 0, 0), second row as (0, 0, 0) and third row as (0, 0, -1). Now, if someone measures Q just after the measurement of P, what is the probability of getting 0 for P and -1 for Q in the respective measurements?

---

# DeepSeek response (via openrouter)



---

# DeepSeek reasoning (via openrouter)

To solve for the given problem, let us first label the given information explicitly.

The state of the system at time $t$ is given by the column matrix:
$$
\binom{-1}{2}{\mathbf \Psi} = \begin{bmatrix} -1 \\ 2 \\ 1\end{bmatrix}.
$$
The matrix corresponding to the operator $P$ is given as:
$$
\mathbf{P} = \begin{bmatrix}
0 & \frac{1}{\sqrt{2}} & 0 \\
\frac{1}{\sqrt{2}} & 0 & \frac{1}{\sqrt{2}} \\
0 & \frac{1}{\sqrt{2}} & 0
\end{bmatrix}.
$$
Similarly, the matrix corresponding to the operator $Q$ is:
$$
\mathbf{Q} = \begin{bmatrix}
1 & 0 & 0 \\
0 & 0 & 0 \\
0 & 0 & -1
\end{bmatrix}.
$$
The goal is to find the probability that if someone measures $P$ followed by measuring $Q$, one needs to find the probability of getting $0$ for $P$ and then subsequently getting $ -1$ for $Q$.

#### Step 1: Normalize the given state vector.

First, we need to ensure that the given state vector $\mathbf{\Psi} = \begin{bmatrix} -1 \\ 2 \\ 1 \end{bmatrix}$ is normalized. The norm squared of the state vector is given by:
$$
\|\mathbf{\Psi}\|^2 = \begin{bmatrix} -1 & 2 & 1 \end{bmatrix} \begin{bmatrix} -1 \\ 2 \\ 1\end{bmatrix} = (-1)^2 + 2^2 + 1^2 = 1 + 4 + 1 = 6.
$$
The normalized state vector thus is:
$$
|\psi\rangle = \frac{1}{\sqrt{6}} \begin{bmatrix} -1 \\ 2 \\ 1\end{bmatrix} = \frac{1}{\sqrt{6}} \begin{bmatrix} -1 \\ 2 \\ 1\end{bmatrix}.
$$

#### Step 2: Solve for the eigenvalues and eigenvectors of $P$.

To find the eigenvalues $\lambda$ of $P$, we need to solve the characteristic equation $\det(P - \lambda I) = 0$:
$$
\mathbf{P} - \lambda\mathbf{I} = \begin{bmatrix} -\lambda & \frac{1}{\sqrt{2}} & 0 \\
\frac{1}{\sqrt{2}} & -\lambda & \frac{1}{\sqrt{2}} \\
0 & \frac{1}{\sqrt{2}} & -\lambda
\end{bmatrix}.
$$
We compute the determinant:
$$
\det(P - \lambda I) = \det\begin{bmatrix} -\lambda & \frac{1}{\sqrt{2}} & 0 \\
\frac{1}{\sqrt{2}} & -\lambda & \frac{1}{\sqrt{2}} \\
0 & \frac{1}{\sqrt{2}} & -\lambda
\end{bmatrix} = -\lambda \det\begin{bmatrix} -\lambda & \frac{1}{\sqrt{2}} \\
\frac{1}{\sqrt{2}} & -\lambda
\end{bmatrix} - \frac{1}{\sqrt{2}} \det\begin{bmatrix} \frac{1}{\sqrt{2}} & \frac{1}{\sqrt{2}} \\
0 & -\lambda
\end{bmatrix}.
$$
Expanding the two $2 \times 2$ determinants:
$$
\det\begin{bmatrix} -\lambda & \frac{1}{\sqrt{2}} \\
\frac{1}{\sqrt{2}} & -\lambda
\end{bmatrix} = (-\lambda)(-\lambda) - \left(\frac{1}{\sqrt{2}}\right) \left(\frac{1}{\sqrt{2}}\right) = \lambda^2 - \frac{1}{2}.
$$
$$
\det\begin{bmatrix} \frac{1}{\sqrt{2}} & \frac{1}{\sqrt{2}} \\
0 & -\lambda
\end{bmatrix} = -\lambda \cdot \frac{1}{\sqrt{2}}.
$$
Therefore:
$$
\det(P - \lambda I) = -\lambda\left(\lambda^2 - \frac{1}{2}\right) - \frac{1}{\sqrt{2}}\left(-\lambda \cdot \frac{1}{\sqrt{2}}\right) = -\lambda\left(\lambda^2 - \frac{1}{2}\right) + \frac{\lambda}{2} = -\lambda^3 + \frac{\lambda}{2} + \frac{\lambda}{2} = -\lambda^3 + \lambda = -\lambda(\lambda^2 - 1).
$$
Thus solving for the characteristic equation:
$$
\lambda(\lambda^2 - 1) = 0.
$$
The eigenvalues are $\lambda = 0, 1,$ and $-1$.

#### Step 3: Find the eigenvectors corresponding to these eigenvalues for $P$.

For $\lambda = 1$:
$$
\begin{bmatrix}
0 & \frac{1}{\sqrt{2}} & 0 \\
\frac{1}{\sqrt{2}} & 0 & \frac{1}{\sqrt{2}} \\
0 & \frac{1}{\sqrt{2}} & 0
\end{bmatrix}
\begin{bmatrix} x \\ y \\ z \end{bmatrix} = 1 \begin{bmatrix} x \\ y \\ z \end{bmatrix}.
$$
This leads to the system of equations:
$$
\frac{1}{\sqrt{2}} y = x,
$$
$$
\frac{1}{\sqrt{2}} x + \frac{1}{\sqrt{2}} z = y,
$$
$$
\frac{1}{\sqrt{2}} y = z.
$$
From $\frac{1}{\sqrt{2}} y = x$, we write $x = \frac{y}{\sqrt{2}}$, and from $\frac{1}{\sqrt{2}} $ y = z$, we write $z = \frac{y}{\sqrt{2}}$. Thus, an eigenvector corresponding to eigenvalue $\lambda = 1$ has the form:
$$
\begin{bmatrix} x \\ y \\ z \end{bmatrix} = \begin{bmatrix}{} \frac{y}{\sqrt{2}} \\ y \\ \frac{y}{\sqrt{2}} \end{bmatrix}.
$$
Choosing $y = \sqrt{2}$ yields:
$$
\begin{bmatrix} 1 \\ \sqrt{2} \\ 1 \end{bmatrix}.
$$
Normalizing this vector requires us to compute its norm:
$$
\|(1, \sqrt{2}, 1)\|^2 = 1^2 + (\sqrt{2})^2 + 1^2 = 1 + 2 + 1 = 4.
$$
The normalized eigenvector for $\lambda = 1$ thus is:
$$
|p_1\rangle = \frac{1}{2} \begin{bmatrix} 1 \\ \sqrt{2} \\ 1 \end{bmatrix} = \begin{bmatrix} 0.5 \\ \frac{\sqrt{2}}{2} \\ 0.5 \end{bmatrix} = \begin{bmatrix} \frac{1}{2} \\ \frac{1}{\sqrt{2}} \\ \frac{1}{2} \end{bmatrix}.
$$
We verify normalization:
$$
\left(\frac{1}{2}\right)^2 + \left(\frac{1}{\sqrt{2}}\right)^2 + \left(\frac{1}{2}\right)^2 = \frac{1}{4} + \frac{1}{2} + \frac{1}{4} = 1.
$$
So:
$$
|p_1\rangle = \frac{1}{2} \begin{bmatrix} 1 \\ \sqrt{2} \\ 1 \end{bmatrix}.
$$

For $\lambda = -1$:
$$
\begin{bmatrix}
0 & \frac{1}{\sqrt{2}} & 0 \\
\frac{1}{\sqrt{2}} & 0 & \frac{1}{\sqrt{2}}\\
0 & \frac{1}{\sqrt{2}} & 0 \\
\end{bmatrix}
\begin{bmatrix} x \\ y \\ z \end{bmatrix} = -1 \begin{bmatrix} x \\ y \\ z \end{bmatrix}.
$$
This generates another set of equations:
$$
\frac{1}{\sqrt{2}} y = -x,
$$
$$
\frac{1}{\sqrt{2}} x + \frac{1}{\sqrt{2}} z = - y,
$$
$$
\frac{1}{\sqrt{2}} y = -z.
$$
This implies $x = -\frac{y}{\sqrt{2}}$ and $z = -\frac{y}{\sqrt{2}}$. Another eigenvector corresponding to eigenvalue $\lambda = -1$ thus has the form:
$$
\begin{bmatrix} x \\ y \\ z \end{bmatrix} = \begin{bmatrix} -\frac{y}{\sqrt{2}} \\ y \\ -\frac{y}{\sqrt{2}} \end{bmatrix}.
$$
Choosing $y = \sqrt{2}$ yields:
$$
\begin{bmatrix} -1 \\ \sqrt{2} \\ -1 \end{bmatrix}.
$$
Normalizing this eigenvector requires us to compute its norm:
$$
\|(-1, \sqrt{2}, -1)\|^2 = (-1)^2 + (\sqrt{2})^2 + (-1)^2 = 1 + 2 + 1 = 4.
$$
The normalized eigenvector for $\lambda = -1$ thus is:
$$
|p_{-1\rangle} = \frac{1}{2} \begin{bmatrix} -1 \\ \sqrt{2} \\ -1\end{bmatrix} = \begin{bmatrix} -0.5 \\ -\frac{\sqrt{2}}{2} \\ 0.5 \end{bmatrix} = \begin{bmatrix} -\frac{1}{2} \\ \frac{1}{\sqrt{2}} \\ -\frac{1}{2} \end{bmatrix} .
$$
Verifying normalization:
$$
\left(\frac{-1}{2}\right)^2 + \left(\frac{1}{\sqrt{2}}\right)^2 + \left(\frac{-1}{2}\right)^2 = \\
\frac{1}{4} + \frac{1}{2} + \frac{1}{4} = 1.
$$
So:
$$
|p_{-1\rangle} = \frac{1}{2}\begin{bmatrix} -1 \\ \sqrt{2} \\ -1 \end{bmatrix}.
$$

For $\lambda = 0$:
$$
\begin_{bmatrix}
0 & \frac{1}{\sqrt{2}} & 0 \\
\frac{1}{\sqrt{2}} & 0 & \frac{1}{\sqrt{2}}\\
0 & \frac{1}{\sqrt{2}} & 0 \\
\end{bmatrix}
\begin{bmatrix} x \\ y \\ z \end{bmatrix} = 0 \begin{bmatrix} x \\ y \\ z \end{bmatrix}.
$$
This generates the system:
$$
\frac{1}{\sqrt{2}} y = 0,
$$
$$
\frac{1}{\sqrt{2}} x + \frac{1}{\sqrt{2}} z = 0,
$$
$$
\frac{1}{\sqrt{2}} y = 0.
$$
Thus $ y=0$, $x = -z$. An eigenvector thus has the form:
$$
\begin{bmatrix} x \\ y \\ z \end{bmatrix} = \begin{bmatrix} \\ 0 \\ -x \end{bmatrix},
$$
where $z = -x$. Thus, if we choose $x = 1$, $z = -1$ yields:
$$
\begin{bmatrix} 1 \\ 0 \\ -1 \end{bmatrix}.
$$
The norm of this vector is:
$$
\|(1, 0, -1)\| ^2 = 1^2 + 0^2 + (-1)^2 = 1 + 1 = 2.
$$
The normalized eigenvector for $\lambda = 0$ thus is:
$$
|p_0\rangle = \frac{1}{\sqrt{2}}\begin{bmatrix} 1 \\ 0 \\ -1 \end{bmatrix} = \begin{bmatrix}\frac{1}{\sqrt{2}} \\ 0 \\ \frac{-1}{\sqrt{2}} \end{bmatrix}.
$$
Verify normalization:
$$
\left(\frac{1}{\sqrt{2}}\right)^2 + 0 + \left(\frac{-1}{\sqrt{2}}\right)^2 = \frac{1}{2} + \frac{1}{2} = 1.
$$
So:
$$
|p_0\rangle = \frac{1}{\sqrt{2}} \begin{bmatrix} 1 \\ 0 \\ -1 \end{bmatrix}.
$$

#### Exact orthogonality check:

To check orthogonality, the inner products should be calculated:
$$
\langle p_1|p_{-1}\rangle = \left(\frac{1}{2} \begin{bmatrix} 1 & \sqrt{2} & 1\end{bmatrix}\right) \left(\frac{1}{2} \begin{bmatrix} -1 \\ \sqrt{2} \\ -1 \end{bmatrix}\right) = \tfrac{1}{4} \left(1 \times (-1) + \sqrt{2} \times \sqrt{2} + 1 \times (-1)\right) = \tfrac{1}{4} (-1 + 2 -1) = 0,
$$
$$
\langle p_1|p_0\rangle = \left(\frac{1}{2} \begin{bmatrix} 1 &\sqrt{2} & 1 \end{bmatrix}\right) \left(\frac{1}{\sqrt{2}}\begin{bmatrix} 1 \\ 0 \\ -1 \end{bmatrix}\right) = \tfrac{1}{2\sqrt{2}} (1 \times 1 + \sqrt{2}\times 0 + 1 \times (-1)) = \tfrac{1}{\sqrt{2}} (1 - + 0 - 1) = 0,
$$
$$
\langle p_{_{-1}}|p_0\rangle = \left(\frac{1}{2}\begin{bmatrix} -1 & \sqrt{2} & -1 \end{bmatrix}\right) \left(\frac{1}{\sqrt{2}}\begin{bmatrix} 1 \\ 0 \\ -1 \end{bmatrix}\right) = \tfrac{1}{2\sqrt{2}}(-1 \times 1 + sqrt{2} \times 0 + (-1) \times (-1)) = \tfrac{1}{2\sqrt{2}} (-1 + 0 + 1) = 0.
$$
This confirms orthogonal eigenvectors.

#### Step 4: Solve for eigenvalues and eigenvectors for $Q$ matrix.

For matrix $Q$:
$$
\mathbf{Q} = \begin{bmatrix}
1 & 0 & 0 \\
0 & 0 & 0 \\
0 & 0 & -1 
\end{bmatrix}.
$$
The characteristic equation is:
$$
\det(Q - \lambda I) = \det\begin{bmatrix}
1 - \lambda & 0 & 0 \\
0 & -\lambda & 0 \\
0 & 0 & -1 - \lambda
\end{bmatrix} = (1 - \lambda)(-\lambda)(-1 - \lambda) = 0,
$$
which directly yields eigenvalues $\lambda = 1, 0,$ and $-1$.

To find the eigenvectors:
For $\lambda = 1$:
$$
\begin{bmatrix}
1 & 0 & 0 \\
0 & 0 & 0 \\
0 & 0 & -1
\end{bmatrix}
\begin{bmatrix} x \\ y \\ z \end{bmatrix} = \begin{bmatrix} x \\ y \\ z\end{bmatrix}.
$$
$$
\begin{bmatrix} x \\ 0 \\ -z \end{bmatrix} = \begin{bmatrix} x \\ y \\ z \endeldbracket.
$$
Hence $x = x$, $0 = y$, and $ -z = z$, implying $z = 0$. An eigenvector for $\lambda = 1$ has the form:
$$
\begin{bmatrix} x \\ \ 0 \\ 0 \end{bmatrix}.
$$
Normalized state has unit norm ($x = 1$):
$$
|q_1\rangle = \begin{bmatrix} 1 \\ 0 \\ 0 \end{bmatrix}.
$$
Verify norm:
$$
\left\| \begin{bmatrix} 1 \\ 0 \\ {0} \end{bmatrix}\right\|^2 = 1 + 0 + 0 = \,1.
$$
Thus:
$$
|q_1\rangle = \begin{bmatrix} 1 \\ 0 \\ 0 \end{bmatrix}.
$$
Similarly, for $\lambda = 0$:
$$
\begin{bmatrix}
1 & 0 & 0 \\
0 & 0 & 0 \\
0 & 0 & -1
\end{bmatrix}
\begin{bmatrix} x \\ y \\ \ z \end{bmatrix} = 0\begin{bmatrix} x \\ y \\ z \end{bmatrix}.
$$
This yields:
$$
\begin{bmatrix} x \\ 0 \\ -z \end{bmatrix} = \begin{bmatrix} \\ z \end{bmatrix}.
$$
Hence $x = 0$ and $z = $. Therefore, an eigenvector for eigenvalue $0$ has the form:
$$
\begin{bmatrix} 0 \\ y \\ 0 \end	local{bmatrix}.
$$
Choosing $y = 1$, so $y = 1$, the normalized state vector ($y = 1$ makes the norm already equals one):
$$
|q_0\rangle = \begin{bmatrix} 0 \\ 1 \\ 0 \end{bmatrix}.
$$
Verify norm:
$$
\left\| \begin{bmatrix} 0 \\ 1 \\ 0 \end{bmatrix} \right\|^2 = 0^{2} + 1^2USTOM 0 = 1.
$$
So indeed:
$$
|q_0\rangle = \begin{bmatrix} 0 \\ 1 \\ 0 \end{bmatrix}.
$$

For $\lambda = -1$:
$$
\begin{bmatrix}  disclaimer\\
1 & 0      & 0 \\
0 & 0  & 0 \\
0 & uddled 0 & -1
\end{bmatrix}
\begin{bmatrix} x \\ y \\ z \end{bmatrix}给自己的 = -1 \begin{bmatrix} x \\ y \\ z \end{bmatrix}.
$$
This yields:
$$
	\begin{bmatrix} x \\ 0 \\ -初三 价 \end{bmatrix} = \begin[{-x \\ -	y \\ -z \end在用{bmatrix].
$$
This leads to $x = -x$, $0 = -y$, and $-z = -z$, hence $x = 0$$0 = -y$, and $z等= z$. Consequently, $ x = 0 (= 杀戮)= 0$, and启垦 an eigenvector for $\lambda耙牛了 = -1$ has the form:
$$
\begin{bmatrix} 0 \\ 0 \\ z \end{bmatrix}.
$$
Read an $z = 1$, the eigenvector becomes:
$$
\begin{bmatrix} 0 \\ 0 \\ tud1 \end{bmatrix}.
$$
Verify norm:
$$
\left\| \begin{bmatrix下学期 0 \\ 0 \\ profession1 \end{bmatrix} \right\|^2 = 0^2 +\虎nm 0鉴于 += 1.
-summarizing have:
$$
|q_{-1}\rangle = \begin{bmatrix} 0 \\ 0 \\ 1 \end{bmatrix}.
$$

#### Step 5: Decompile the initial state in terms of eigenstates of $P算子分解器实操。

Recalling the eigenstates surveyed:
$$
|p_1\rangle = \frac{1}{2} \begin{bmatrix} 1 \\ \sqrt故名ilateral} \\ 1

---

