# Original Question

The state of a system at time t is given by the column matrix having elements (-1, 2, 1). An observable of the system is represented by the matrix operator P having elements in the first row as (0, 1/ \sqrt{2}, 0),  in the second row as (1/ \sqrt{2}, 0, 1/ \sqrt{2}) and in the third row as (0, 1/ \sqrt{2}, 0). Calculate the probability that the measurement of the observable will yield 0 at time t.

---

# DeepSeek response (via openrouter)

\boxed{\frac{1}{3}}

---

# DeepSeek reasoning (via openrouter)

To solve for the probability that a measurement of the observable represented by the matrix $P$ will yield the eigenvalue $0$ at time $t$, we need to follow these steps:

1. Normalize the given state vector.
2. Diagonalize the matrix $P$ to find its eigenvalues and eigenvectors.
3. Project the normalized state vector onto the eigenspace corresponding to the eigenvalue $0$ (if it exists).
4. The probability that a measurement of $P$ yields $0$ is given by the square of the norm of this projection.

The given state of the system at time $t$ is represented by the column matrix:
$$
|\psi\rangle = \begin{pmatrix} -1 \\ 2 \\ 1 \end{pmatrix}.
$$
The given matrix $P$ representing an observable is:
$$
P = \begin{pmatrix}
0 & \frac{1}{\sqrt{2}} & 0 \\
\frac{1}{\sqrt{2}} & 0 & \frac{1}{\sqrt{2}} \\
0 & \frac{1}{\sqrt{2}} & 0
\end{pmatrix}.
$$
The question asks us to find the probability that a measurement of $P$ will yield the value $0$ at time $t$.

#### Step 1: Normalize the state vector $|\psi\rangle$

The norm of $|\psi\rangle$ is given by:
$$
\|\psi\| = \sqrt{\langle\psi|\psi\rangle} = \sqrt{(-1)^2 + 2^2 + 1^2} = \sqrt{1 + 4 + 1} = \sqrt{6}.
$$
The normalized state vector $|\psi_{\text{norm}}\rangle$ is thus:
$$
|\psi_{\text{norm}}\rangle = \frac{1}{\sqrt{6}} \begin{pmatrix} -1 \\ 2 \\ 1 \end{pmatrix} = \begin{pmatrix} \frac{-1}{\sqrt{6}} \\ \frac{2}{\sqrt{6}} \\ \frac{1}{\sqrt{6}} \end{pmatrix} = \begin{pmatrix} -\frac{1}{\sqrt{6}} \\ \frac{2}{\sqrt{6}} \\ \frac{1}{\sqrt{6}} \end{pmatrix}.
$$
(Note that the normalized state vector can be written as $|\psi_{\text{norm}}\rangle = \frac{1}{\sqrt{6}}(-1, 2, 1)^T$.)

#### Step 2: Find the eigenvalues and eigenvectors of $P$

To find the eigenvalues $\lambda$ of $P$, we solve the characteristic equation:
$$
\det(P - \lambda I) = 0,
$$
where $I$ is the $3 \times 3$ identity matrix. Thus, we need to solve:
$$
\det \begin{pmatrix}
-\lambda & \frac{1}{\sqrt{2}} & 0 \\
\frac{1}{\sqrt{2}} & -\lambda & \frac{1}{\sqrt{2}} \\
0 & \frac{1}{\sqrt{2}} & -\lambda
\end{pmatrix} = 0.
$$
Expanding the determinant:
$$
\det \begin{pmatrix}
-\lambda & \frac{1}{\sqrt{2}} & 0 \\
\frac{1}{\sqrt{2}} & -\lambda & \frac{1}{\sqrt{2}} \\
0 & \frac{1}{\sqrt{2}} & -\lambda
\end{pmatrix} = -\lambda \det \begin{pmatrix} -\lambda & \frac{1}{\sqrt{2}} \\ \frac{1}{\sqrt{2}} & -\lambda \end{pmatrix} - \frac{1}{\sqrt{2}} \det \begin{pmatrix} \frac{1}{\sqrt{2}} & \frac{1}{\sqrt{2}} \\ 0 & -\lambda \end{pmatrix} + 0 \cdot \det \begin{pmatrix} \frac{1}{\sqrt{2}} & -\lambda \\ 0 & \frac{1}{\sqrt{2}} \end{pmatrix}.
$$
The first $2 \times 2$ determinant is:
$$
\det \begin{pmatrix} -\lambda & \frac{1}{\sqrt{2}} \\ \frac{1}{\sqrt{2}} & -\lambda \end{pmatrix} = (-\lambda)(-\lambda) - \left(\frac{1}{\sqrt{2}}\right)\left(\frac{1}{\sqrt{2}}\right) = \lambda^2 - \frac{1}{2}.
$$
The second $2 \times 2$ determinant is:
$$
\det \begin{pmatrix} \frac{1}{\sqrt{2}} & \frac{1}{\sqrt{2}} \\ 0 & -\lambda \end{pmatrix} = \left(\frac{1}{\sqrt{2}}\right)(-\lambda) - \left(\frac{1}{\sqrt{2}}\right) \cdot 0 = -\frac{\lambda}{\sqrt{2}}.
$$
The third $2 \times 2$ determinant is not needed because it is multiplied by $0$. Thus, the characteristic equation becomes:
$$
-\lambda \left(\lambda^2 - \frac{1}{2}\right) - \frac{1}{\sqrt{2}} \left(-\frac{\lambda}{\sqrt{2}}\right) = 0,
$$
which simplifies to:
$$
-\lambda \left(\lambda^2 - \frac{1}{2}\right) + \frac{\lambda}{2} = 0,
$$
$$
-\lambda \left(\lambda^2 - \frac{1}{2} - \frac{1}{2}\right) = 0,
$$
$$
-\lambda \left(\lambda^2 - 1\right) = 0,
$$
$$
-\lambda(\lambda - 1)(lambda + 1) = 0.
$$
The eigenvalues are thus:
$$
\lambda = 0, \ 1, \ -1.
$$
We need to find the eigenvectors for each eigenvalue.

#### For $\lambda = 0$:
$$
\begin{pmatrix}
0 & \frac{1}{\sqrt{2}} & 0 \\
\frac{1}{\sqrt{2}} & 0 & \frac{1}{\sqrt{2}} \\
0 & \frac{1}{\sqrt{2}} & 0
\end{pmatrix} \begin{pmatrix} a \\ b \\ c \end{pmatrix} = 0 \begin{pmatrix} a \\ b \\ c \end{pmatrix} = \begin{pmatrix} 0 \\ 0 \\ 0 \end{pmatrix}.
$$
This leads to the system of equations:
$$
\frac{1}{\sqrt{2}}b = 0,
$$
$$
\frac{1}{\sqrt{2}}a + \frac{1}{\sqrt{2}}c = 0,
$$
$$
\frac{1}{\sqrt{2}}b = 0.
$$
The first and third equations both give $b = 0$. The second equation gives $a + c = 0$, so $a = -c$. Thus, an eigenvector for $\lambda = 0$ can be written as:
$$
\begin{pmatrix} a \\ 0 \\ -a \end{pmatrix} = a \begin{pmatrix} 1 \\ 0 \\ -1 \end{pmatrix}.
$$
Normalizing this eigenvector (i.e., making sure it has a norm of $1$):
$$
\left\|\begin{pmatrix} 1 \\ 0 \\ -1 \end{pmatrix}\right\| = \sqrt{1^2 + 0^2 + (-1)^2} = \sqrt{2}.
$$
The normalized eigenvector for $\lambda = 0$ is thus:
$$
|0\rangle = \frac{1}{\sqrt{2}} \begin{pmatrix} 1 \\ 0 \\ -1 \end{pmatrix} = \begin{pmatrix} \frac{1}{\sqrt{2}} \\ 0 \\ -\frac{1}{\sqrt{2}} \end{pmatrix}.
$$

#### For $\lambda = 1$:
$$
\begin{pmatrix}
0 & \frac{1}{\sqrt{2}} & 0 \\
\frac{1}{\sqrt{2}} & 0 & \frac{1}{\sqrt{2}} \\
0 & \frac{1}{\sqrt{2}} & 0
\end{pmatrix} \begin{pmatrix} a \\ b \\ c \end{pmatrix} = 1 \begin{pmatrix} a \\ b \\ c \end{pmatrix} = \begin{pmatrix} a \\ b \\ c \end{pmatrix}.
$$
This leads to the system of equations:
$$
\frac{1}{\sqrt{2}}b = a,
$$
$$
\frac{1}{\sqrt{2}}a + \frac{1}{\sqrt{2}}c = b,
$$
$$
\frac{1}{\sqrt{2}}b = c.
$$
The first equation gives $b = \sqrt{2}a$, and the third equation gives $b = \sqrt{2}c$. Thus, $a = c$ and $b = \sqrt{2}a$. An eigenvector for $\lambda = 1$ can be written as:
$$
\begin{pmatrix} a \\ \sqrt{2}a \\ a \end{pmatrix} = a \begin{pmatrix} 1 \\ \sqrt{2} \\ 1 \end{pmatrix}.
$$
Normalizing this eigenvector:
$$
\left\|\begin{pmatrix} 1 \\ \sqrt{2} \\ 1 \end{pmatrix}\right\| = \sqrt{1^2 + (\sqrt{2})^2 + 1^2} = \sqrt{1 + 2 + 1} = 2.
$$
The normalized eigenvector for $\lambda = 1$ is thus:
$$
|1\rangle = \frac{1}{2} \begin{pmatrix} 1 \\ \sqrt{2} \\ 1 \end{pmatrix} = \begin{pmatrix} \frac{1}{2} \\ \frac{\sqrt{2}}{2} \\ \frac{1}{2} \end{pmatrix} = \begin{pmatrix} \frac{1}{2} \\ \frac{1}{\sqrt{2}} \\ \frac{1}{2} \end{pmatrix}.
$$

#### For $\lambda = -1$:
$$
\begin{pmatrix}
0 & \frac{1}{\sqrt{2}} & 0 \\
\frac{1}{\sqrt{2}} & 0 & \frac{1}{\sqrt{2}} \\
0 & \frac{1}{\sqrt{2}} & 0
\end{pmatrix} \begin{pmatrix} a \\ b \\ c \end{pmatrix} = -1 \begin{pmatrix} a \\ b \\ c \end{pmatrix} = \begin{pmatrix} -a \\ -b \\ -c \end{pmatrix}.
$$
This leads to the system of equations:
$$
\frac{1}{\sqrt{2}}b = -a,
$$
$$
\frac{1}{\sqrt{2}}a + \frac{1}{\sqrt{2}}c = -b,
$$
$$
\frac{1}{\sqrt{2}}b = -c.
$$
The first equation gives $b = -\sqrt{2}a$, and the third equation gives $b = -\sqrt{2}c$. Thus, $a = c$ and $b = -\sqrt{2}a$. An eigenvector for $\lambda = -1$ can be written as:
$$
\begin{pmatrix} a \\ -\sqrt{2}a \\ a \end{pmatrix} = a \begin{pmatrix} 1 \\ -\sqrt{2} \\ 1 \end{pmatrix}.
$$
Normalizing this eigenvector:
$$
\left\|\begin{pmatrix} 1 \\ -\sqrt{2} \\ 1 \end{pmatrix}\right\| = \sqrt{1^2 + (-\sqrt{2})^2 + 1^2} = \sqrt{1 + 2 + 1} = 2.
$$
The normalized eigenvector for $\lambda = -1$ is thus:
$$
|-1\rangle = \frac{1}{2} \begin{pmatrix} 1 \\ -\sqrt{2} \\ 1 \end{pmatrix} = \begin{pmatrix} \frac{1}{2} \\ -\frac{\sqrt{2}}{2} \\ \frac{1}{2} \end{pmatrix} = \begin{pmatrix} \frac{1}{2} \\ -\frac{1}{\sqrt{2}} \\ \frac{1}{2} \end{pmatrix}.
$$

#### Step 3: Project the normalized state vector onto the eigenspace corresponding to the eigenvalue $0$

The normalized state vector is:
$$
|\psi_{\text{norm}}\rangle = \begin{pmatrix} -\frac{1}{\sqrt{6}} \\ \frac{2}{\sqrt{6}} \\ \frac{1}{\sqrt{6}} \end{pmatrix}.
$$
The only eigenvector for the eigenvalue $0$ is:
$$
|0\rangle = \begin{pmatrix} \frac{1}{\sqrt{2}} \\ 0 \\ -\frac{1}{\sqrt{2}} \end{pmatrix}.
$$
The probability that a measurement of $P$ yields $0$ is given by the square of the inner product (i.e., the "overlap") between $|\psi_{\text{norm}}\rangle$ and $|0\rangle$:
$$
\langle0|\psi_{\text{norm}}\rangle = \left(\frac{1}{\sqrt{2}}, 0, -\frac{1}{\sqrt{2}}\right) \begin{pmatrix} -\frac{1}{\sqrt{6}} \\ \frac{2}{\sqrt{6}} \\ \frac{1}{\sqrt{6}} \end{pmatrix} = \frac{1}{\sqrt{2}} \cdot \left(-\frac{1}{\sqrt{6}}\right) + 0 \cdot \frac{2}{\sqrt{6}} + \left(-\frac{1}{\sqrt{2}}\right) \cdot \frac{1}{\sqrt{6}}.
$$
$$
= \frac{1}{\sqrt{2}} \cdot \left(-\frac{1}{\sqrt{6}}\right) - \frac{1}{\sqrt{2}} \cdot \frac{1}{\sqrt{6}} = -\frac{1}{\sqrt{12}} - \frac{1}{\sqrt{12}} = -\frac{1}{\sqrt{12}} - \frac{1}{\sqrt{12}} = -\frac{2}{\sqrt{12}} = -\frac{2}{2\sqrt{3}} = -\frac{1}{\sqrt{3}} = -\frac{\sqrt{3}}{3}.
$$
The probability is the square of the absolute value of this inner product:
$$
|\langle0|\psi_{\text{norm}}\rangle|^2 = \left|-\frac{\sqrt{3}}{3}\right)^2 = \left(\frac{\sqrt{3}}{3}\right)^2 = \left(\frac{\sqrt{3}}{3}\right)^2 = \frac{3}{9} = \frac{1}{3}.
$$

#### Conclusion:
The probability that a measurement of the observable $P$ will yield the value $0$ at time $t$ is:
$$
\boxed{\frac{1}{3}}.
$$

#### Verification of the inner product calculation:
To make sure the inner product calculation is verified explicitly:
$$
\langle0|\psi_{\text{norm}}\rangle = \left(\frac{1}{\sqrt{2}}, 0, -\frac{1}{\sqrt{2}}\right) \begin{pmatrix} -\frac{1}{\sqrt{6}} \\ \frac{2}{\sqrt{6}} \\ \frac{1}{\sqrt{6}} \end{pmatrix} = \left(\frac{1}{\sqrt{2}}\right) \left(-\frac{1}{\sqrt{6}}\right) + 0 \cdot \left(\frac{2}{\sqrt{6}}\right) + \left(-\frac{1}{\sqrt{2}}\right) \left(\frac{1}{\sqrt{6}}\right) = -\frac{1}{\sqrt{12}} + 0 - \frac{1}{\sqrt{12}} = -\frac{1}{\sqrt{12}} - \frac{1}{\sqrt{12}}.
$$
$$
= -\frac{1}{2\sqrt{3}} - \frac{1}{2\sqrt{3}} = -\frac{1}{\sqrt{12}} - \frac{1}{\sqrt{12}} = -\frac{2}{\sqrt{12}} = -\frac{2}{2\sqrt{3}} = -\frac{1}{\sqrt{3}} = -\frac{\sqrt{3}}{3}.
$$
The square of the absolute value of this inner product is:
$$
\left|\langle0|\psi_{\text{norm}}\rangle\right|^2 = \left|-\frac{\sqrt{3}}{3}\right|^2 = \left(\frac{\sqrt{3}}{3}\right)^2 = \frac{3}{9} = \frac{1}{3}.
$$

This reasoning makes us confident that the answer is indeed $\frac{1}{3}$.


---

